Reimplements library and adds features
This is an alomost complete reimplemtation of the library.  Moreover,
this version has a complete proof that an EDT0L language is LULT if and
only if it is EDT0L of finite index.

LSystems/EDT0L/Basic.lean
@@ -3,146 +3,204 @@ Copyright (c) 2025 Alex Bishop. All rights reserved.
 Released under Apache 2.0 license as described in the file LICENSE.
 Author: Alex Bishop
 -/
-import LSystems.EDT0L.Defs
+module
+
+public import LSystems.EDT0L.Defs
+
+/-!
+# Basic 
+-/
+
+@[expose] public section
+
+@[simp]
+lemma List.map_terminal {α V} (u v : List α) :
+    u.map (β := Symbol α V) .terminal = v.map .terminal ↔ u = v := by
+  refine map_inj_right ?_
+  simp
 
 namespace EDT0LGrammar
 
 @[simp]
-theorem no_tables_imp_eq_0 {α V T : Type*} [Fintype V] [Fintype T] [IsEmpty T]
-  (E : EDT0LGrammar α V T) :
-    E.language = 0 := by
-  unfold EDT0LGrammar.language
-  have hh (w : List α) : ¬ E.generates (List.map .terminal w) := by
-    intro h
-    unfold EDT0LGrammar.generates at h
-    unfold EDT0LGrammar.derives at h
-    rw [Relation.reflTransGen_iff_eq_or_transGen] at h
-    cases h with
-    | inl h =>
-      simp_all only [List.map_eq_singleton_iff, reduceCtorEq, and_false, exists_false]
-    | inr h =>
-      cases h with
-      | single h => 
-        unfold EDT0LGrammar.rewrites at h
-        simp_all only [IsEmpty.exists_iff]
-      | tail _ h =>
-        unfold EDT0LGrammar.rewrites at h
-        simp_all only [IsEmpty.exists_iff]
-  simp only [hh]
-  simp only [Set.setOf_false]
-  rfl
+theorem no_tables_imp_eq_0 {α V T} [IsEmpty T] (E : EDT0LGrammar α V T) : E.language = 0 := by
+  ext1 w
+  simp only [language_mem_iff, Language.notMem_zero, iff_false]
+  intro contra
+  unfold Generates Derives at contra
+  rw [Relation.reflTransGen_iff_eq_or_transGen] at contra
+  obtain contra | contra := contra
+  · simp_all
+  · cases contra with | single h | tail x h =>
+    obtain ⟨t, h⟩ := h
+    exact IsEmpty.false t
 
-theorem language_0_is_EDT0L {α : Type*} : Language.IsEDT0L (0 : Language α) := by
-  let E : EDT0LGrammar α (Fin 1) (Fin 0) := ⟨ 
-    0,
-    fun _ ↦ fun _ ↦ []
-  ⟩
-  use 1, 0, E, E.no_tables_imp_eq_0
+def zero {α} : EDT0LGrammar α (Fin 1) (Fin 0) where
+  initial := 0
+  table := fun _ _ ↦ []
 
-theorem language_1_is_EDT0L {α : Type*} : Language.IsEDT0L (1 : Language α) := by
-  let E : EDT0LGrammar α (Fin 1) (Fin 1) := ⟨ 
-    0,
-    fun _ ↦ fun _ ↦ []
-  ⟩
-  simp only [Language.IsEDT0L, EDT0LGrammar.language]
+lemma zero_language {α} : zero.language = (0 : Language α) := no_tables_imp_eq_0 zero
 
-  have h : E.derives [.nonterminal E.initial] [] := by
-    unfold EDT0LGrammar.derives
-    apply Relation.ReflTransGen.tail (Relation.ReflTransGen.refl) _
-    use 0
-    subst E
-    simp only [Fin.isValue, rewriteWord_cons, rewriteSymbol_nonterminal, rewriteWord_nil,
-      List.append_nil]
+def one {α} : EDT0LGrammar α (Fin 1) (Fin 1) where
+  initial := 0
+  table := fun _ _ ↦ []
 
-  have h : ∀ w :
-      List (Symbol α (Fin 1)), E.generates w → w = [Symbol.nonterminal 0] ∨ w = [] := by
-    intro w
-    intro h₁
-    rw [EDT0LGrammar.generates, EDT0LGrammar.derives] at h₁
-
-    induction h₁ with
+lemma one_language {α} : one.language = (1 : Language α) := by
+  have go {w : List (Symbol α (Fin 1))} (h : one.Generates w) : w = one.initialWord ∨ w = [] := by
+    induction h with
     | refl =>
-        left
-        simp only [E]
-    | tail h₂ h₃ h₄ =>
+      simp
+    | tail x y ih =>
+      rename_i a b
+      obtain rfl | rfl := ih <;> {
+        simp only [Rewrites, rewriteWord_cons, rewriteSymbol_nonterminal, rewriteWord_nil,
+          List.append_nil, Fin.exists_fin_one, Fin.isValue] at y
+        subst b
         right
-        cases h₄ with
-        | inl h₄ =>
-            rw [h₄] at h₃
-            clear h₄
-            rw [EDT0LGrammar.rewrites] at h₃
-            have h₄ : ∀ τ : (Fin 1), τ = 0 := by
-              --aesop?
-              intro τ
-              simp_all only [Fin.isValue, E]
-              obtain ⟨w_1, h⟩ := h₃
-              subst h
-              ext : 1
-              simp_all only [Fin.isValue, Fin.val_eq_zero]
-            simp only [h₄,exists_const] at h₃ 
-            clear h₄
-            -- rw [EDT0LGrammar.RewriteWord] at h₃
-            --
-            cases h₃ with | refl
-            --
-            -- show_term bound
-            rfl
-        | inr h₄ =>
-            rw [h₄] at h₃
-            clear h₄
-            rw [EDT0LGrammar.rewrites] at h₃
-            have h₄ : ∀ τ : (Fin 1), τ = 0 := by
-              --aesop?
-              intro τ
-              simp_all only [Fin.isValue, E]
-              obtain ⟨w_1, h⟩ := h₃
-              subst h
-              ext : 1
-              simp_all only [Fin.isValue, Fin.val_eq_zero]
-            simp only [EDT0LGrammar.rewriteWord_nil, List.nil_eq, exists_const] at h₃
-            rw [← h₃]
-  -------------------
-  use 1, 1, E
+        rfl }
+  ext1 w
+  simp only [language_mem_iff, Language.mem_one]
+  constructor
+  · intro h
+    replace h := go h
+    obtain h | h := h <;> simp_all
+  · intro h
+    subst h
+    refine derives_single ?_
+    simp only [Rewrites, rewriteWord_cons, rewriteSymbol_nonterminal, rewriteWord_nil,
+      List.append_nil, List.map_nil, Fin.exists_fin_one, Fin.isValue]
+    rfl
 
-  have h₁ (w : List α) :
-      E.generates (List.map Symbol.terminal w) ↔ w = [] := by
-    constructor
-    case mp =>
-      intro w₁
+theorem language_0_isEDT0L {α} : Language.IsEDT0L (0 : Language α) := ⟨1, 0, zero, zero_language⟩
 
-      have h₂ : _ := h (List.map Symbol.terminal w) w₁ 
+theorem language_1_isEDT0L {α} : Language.IsEDT0L (1 : Language α) := ⟨1, 1, one, one_language⟩
 
-      cases h₂ with
-        | inl h₂ =>
-            simp_all only [List.map_eq_singleton_iff, reduceCtorEq, and_false, exists_false]
-        | inr h₂ =>
-            exact List.map_eq_nil_iff.mp h₂
-    case mpr =>
-      intro w₁
-      rw [w₁]
-      rw [EDT0LGrammar.generates,EDT0LGrammar.derives]
-      simp only [List.map_nil]
-      rw [Relation.reflTransGen_iff_eq_or_transGen]
-      right
-      rw [Relation.transGen_iff]
-      left
-      rw [EDT0LGrammar.rewrites]
-      use 0
-      unfold EDT0LGrammar.rewriteWord
-      unfold EDT0LGrammar.rewriteSymbol
-      subst w₁
-      simp_all only [Fin.isValue, List.flatMap_cons, List.flatMap_nil, List.append_nil, E]
-  exact Language.ext_iff.mpr h₁
-  -------------------
+def getNonterminal? {α V} : Symbol α V → Option V
+  | .terminal _ => none
+  | .nonterminal v => some v
 
-variable {α V T : Type*} [Fintype V] [Fintype T]
-variable {E : EDT0LGrammar α V T}
+def filterNonterminals {α V} : List (Symbol α V) → List V := List.filterMap getNonterminal?
+
+@[simp]
+lemma filterNonterminals_nil {α V} : filterNonterminals ([] : List (Symbol α V)) = [] := rfl
+
+@[simp]
+lemma filterNonterminals_cons {α V} (x : Symbol α V) (xs : List (Symbol α V)) :
+    filterNonterminals (x::xs) = 
+      match x with
+      | .terminal _ => filterNonterminals xs
+      | .nonterminal v => v::filterNonterminals xs := by split <;> rfl
+
+@[simp]
+lemma filterNonterminals_terminals {α V} (w : List α) :
+    filterNonterminals (V := V) (w.map .terminal) = [] := by
+  induction w with
+  | nil =>
+    rfl
+  | cons x xs ih =>
+    simp [ih]
+
+@[simp]
+lemma filterNonterminals_append {α V} (x y : List (Symbol α V)) :
+    filterNonterminals (x ++ y) = filterNonterminals x ++ filterNonterminals y :=
+  List.filterMap_append
+
+lemma filterNonterminals_mem_iff {α V} (v : V) (x : List (Symbol α V)) :
+    v ∈ filterNonterminals x ↔ .nonterminal v ∈ x := by
+  induction x with
+  | nil =>
+    simp
+  | cons a as ih =>
+    simp only [filterNonterminals_cons, List.mem_cons]
+    split <;> simp [ih]
+
+@[simp]
+lemma filterNonterminals_count {α V} [DecidableEq α] [DecidableEq V]
+  (v : V) (x : List (Symbol α V)) :
+    (filterNonterminals x).count v = x.count (.nonterminal v) := by
+  induction x with
+  | nil =>
+    rfl
+  | cons x xs ih =>
+    simp only [filterNonterminals_cons, List.count_cons, beq_iff_eq]
+    split
+    · simpa
+    · simpa [List.count_cons]
+
+@[simp]
+lemma filterNonterminals_map_nonterminal {α V} (w : List V) :
+    filterNonterminals (α := α) (w.map .nonterminal) = w := by
+  induction w with
+  | nil => rfl
+  | cons x xs ih => simp [ih]
+
+@[simp]
+lemma filterNonterminals_take_nonterminal {α V} (w : List V) (i) :
+    filterNonterminals (α := α) (List.take i <| w.map .nonterminal) = w.take i := by
+  induction w with
+  | nil => simp
+  | cons x xs ih =>
+    simp only [List.map_cons]
+    cases i with
+    | zero =>
+      simp
+    | succ i =>
+      simp only [List.take_succ_cons, filterNonterminals_cons, List.cons.injEq, true_and] at ⊢ ih
+      simp only [List.take_add_one, List.getElem?_map, filterNonterminals_append] at ih
+      cases hxs : xs[i]? with
+      | none =>
+        simp only [hxs, Option.map_none, Option.toList_none, filterNonterminals_nil,
+          List.append_nil] at ih
+        exact ih
+      | some x' =>
+        simp only [hxs, Option.map_some, Option.toList_some, filterNonterminals_cons,
+          filterNonterminals_nil, List.append_cancel_right_eq] at ih
+        exact ih
+
+lemma filterNonterminals_rewriteWord {α V T} (x : List (Symbol α V)) (E : EDT0LGrammar α V T)
+  (t : T) :
+    filterNonterminals (E.rewriteWord t x) =
+      filterNonterminals (E.rewriteWord t ((filterNonterminals x).map .nonterminal)) := by
+  induction x with
+  | nil =>
+    rfl
+  | cons x xs ih =>
+    simp only [rewriteWord_cons, filterNonterminals_append, filterNonterminals_cons]
+    split <;> simp [ih]
+
+lemma filterNonterminals_rewriteSymbols {α V T} (x : List (Symbol α V)) (E : EDT0LGrammar α V T)
+  (t : T) :
+    filterNonterminals (E.rewriteWord t x) =
+      filterNonterminals (List.flatMap (E.table t) (filterNonterminals x)) := by
+  rw [filterNonterminals_rewriteWord]
+  unfold rewriteWord rewriteSymbol
+  rw [List.flatMap_map]
+
+@[simp]
+lemma filterNonterminals_equivWord {α α' V V'} {equivα : α ≃ α'} {equivV : V ≃ V'}
+  (w : List (Symbol α V)) :
+    filterNonterminals (equivWord equivα equivV w) = (filterNonterminals w).map equivV := by
+  induction w with
+  | nil =>
+    rfl
+  | cons x xs ih =>
+    simp only [equivWord_cons, filterNonterminals_cons, ih]
+    split <;> split <;> simp_all
+
+@[simp]
+lemma filterNonterminals_equivWord_symm {α α' V V'} {equivα : α ≃ α'} {equivV : V ≃ V'}
+  (w : List (Symbol α' V')) :
+    filterNonterminals ((equivWord equivα equivV).symm w) =
+      (filterNonterminals w).map equivV.symm := by
+  rw [equivWord_symm]
+  exact filterNonterminals_equivWord w
+
+variable {α V T : Type*} {E : EDT0LGrammar α V T}
 
 @[simp]
 lemma rewriteWord_nonterminal_mem [BEq (Symbol α V)] [LawfulBEq (Symbol α V)]
-  {w : List (Symbol α V)} {v} {t : T} :
+  {w : List (Symbol α V)} {v t} :
     .nonterminal v ∈ E.rewriteWord t w ↔
-      ∃ (y : V) (_hy : .nonterminal y ∈ w), .nonterminal v ∈ E.tables t y := by
+      ∃ (y : V) (_hy : .nonterminal y ∈ w), .nonterminal v ∈ E.table t y := by
   constructor
   · intro h
     induction w with
@@ -151,33 +209,21 @@ lemma rewriteWord_nonterminal_mem [BEq (Symbol α V)] [LawfulBEq (Symbol α V)]
     | cons a as ih =>
       simp only [rewriteWord_cons, List.mem_append] at h
       obtain h | h := h
-      · cases a
-        · simp only [rewriteSymbol_terminal, List.mem_cons, reduceCtorEq, List.not_mem_nil,
+      · match a with
+        | .terminal a =>
+          simp only [rewriteSymbol_terminal, List.mem_cons, reduceCtorEq, List.not_mem_nil,
             or_self] at h
-        · rename_i y
-          exact ⟨y, List.mem_cons_self, h⟩
-      · replace ⟨y,hy,ih⟩ := ih h
+        | .nonterminal v =>
+          rename_i vv
+          exact ⟨v, List.mem_cons_self, Multiset.mem_coe.mp h⟩
+      · replace ⟨y, hy, ih⟩ := ih h 
         exact ⟨y, List.mem_cons_of_mem a hy, ih⟩
   · intro h
-    obtain ⟨y, hy, h⟩ := h
-    let idx? := w.finIdxOf? (.nonterminal y)
-    cases h₁ : idx?
-    · subst idx?
-      exfalso
-      exact List.finIdxOf?_eq_none_iff.mp h₁ hy
-    · rename_i i
-      subst idx?
-      rw [List.finIdxOf?_eq_some_iff] at h₁
-      obtain ⟨h₁, h₂⟩ := h₁
-      have h₃ : w.take i ++ [w[i]] ++ w.drop (i + 1) = w := by
-        simp only [Fin.getElem_fin, List.take_append_getElem, List.take_append_drop]
-      rw [h₁] at h₃
-      rw [← h₃]
-      simp only [List.append_assoc, List.cons_append, List.nil_append, rewriteWord_append,
-        rewriteWord_cons, rewriteSymbol_nonterminal, List.mem_append]
-      right
-      left
-      exact h
+    replace ⟨y, hy, h⟩ := h
+    obtain ⟨r, s, rfl⟩ := List.mem_iff_append.mp hy
+    simp only [rewriteWord_append, rewriteWord_cons, rewriteSymbol_nonterminal, List.mem_append]
+    right; left
+    exact h
 
 lemma rewriteWord_mem (w : List (Symbol α V)) (x : Symbol α V) (t : T) :
     x ∈ E.rewriteWord t w ↔ ∃ y ∈ w, x ∈ E.rewriteSymbol t y := by
@@ -185,25 +231,16 @@ lemma rewriteWord_mem (w : List (Symbol α V)) (x : Symbol α V) (t : T) :
   · intro h
     induction w with
     | nil =>
-      simp_all only [rewriteWord_nil, List.not_mem_nil]
+      simp only [rewriteWord_nil, List.not_mem_nil] at h
     | cons a as ih =>
-      rename_i a'
-      simp_all only [
-        rewriteWord_cons, List.mem_append, List.mem_cons,
-        exists_eq_or_imp]
-      cases h with
-      | inl h_1 => simp_all only [true_or]
-      | inr h_2 => simp_all only [forall_const, or_true]
+      simp only [rewriteWord_cons, List.mem_append] at h
+      obtain h | h := h
+      · exact List.exists_mem_cons_of as h
+      · exact List.exists_mem_cons_of_exists (ih h)
   · intro h
-    obtain ⟨y, hy, h⟩ := h
-    have ⟨n, hy'⟩ := List.mem_iff_get.mp hy
-    change w[n] = y at hy'
-    have h₁ : w.take n ++ [w[n]] ++ w.drop (n + 1) = w := by
-      simp only [Fin.getElem_fin, List.take_append_getElem, List.take_append_drop]
-    simp only [hy'] at h₁
-    rw [← h₁]
-    simp only [List.append_assoc, List.cons_append, List.nil_append, rewriteWord_append,
-      rewriteWord_cons, List.mem_append]
+    replace ⟨y, hy, h⟩ := h
+    obtain ⟨r, s, rfl⟩ := List.mem_iff_append.mp hy
+    simp only [rewriteWord_append, rewriteWord_cons, List.mem_append]
     right; left
     exact h
 
