LSystems/EDT0L/DeadEnds.lean
@@ -3,91 +3,58 @@ Copyright (c) 2025 Alex Bishop. All rights reserved.
 Released under Apache 2.0 license as described in the file LICENSE.
 Author: Alex Bishop
 -/
-import LSystems.EDT0L.Defs
+module
+
+public import LSystems.EDT0L.Defs
+
+@[expose] public section
 
 namespace EDT0LGrammar
-variable {α V T : Type*} [Fintype V] [Fintype T] (E : EDT0LGrammar α V T)
 
-def HasDeadEnds (dead : Finset V) : Prop :=
-  ∀ 𝔡 ∈ dead, ∀ t : T, ∃ 𝔡' ∈ dead, .nonterminal 𝔡' ∈ E.tables t 𝔡
+def IsDeadEndSet {α V T} (E : EDT0LGrammar α V T) (dead : Set V) : Prop :=
+  ∀ 𝔡 ∈ dead, ∀ t : T, ∃ 𝔡' ∈ dead, .nonterminal 𝔡' ∈ E.table t 𝔡
 
-def DeadWord (w : List (Symbol α V)) : Prop :=
-  ∃ dead : Finset V, ∃ _ : E.HasDeadEnds dead, ∃ 𝔡 ∈ dead, .nonterminal 𝔡 ∈ w
+def IsDeadEndSingleton {α V T} (E : EDT0LGrammar α V T) (𝔡 : V) : Prop := E.IsDeadEndSet {𝔡}
 
-lemma dead_end_singleton (𝔡 : V) (h : ∀ t : T, .nonterminal 𝔡 ∈ E.tables t 𝔡) :
-    E.HasDeadEnds {𝔡} :=
-  --
-  fun n h τ ↦ ⟨n, h, by simp_all only [Finset.mem_singleton]⟩
+def IsDeadWord {α V T} (E : EDT0LGrammar α V T) (w : List (Symbol α V)) : Prop :=
+  ∃ (dead : Set V) (_ : E.IsDeadEndSet dead) (𝔡 : V) (_ : 𝔡 ∈ dead), .nonterminal 𝔡 ∈ w
 
-lemma rewrite_word_dead_end (w : List (Symbol α V)) (t : T) (dead : Finset V)
-  (h₁ : E.HasDeadEnds dead)
-  (h₂ : ∃ 𝔡 ∈ dead, .nonterminal 𝔡 ∈ w) :
-    ∃ 𝔡' ∈ dead, .nonterminal 𝔡' ∈ E.rewriteWord t w := by
-  replace ⟨𝔡, h₃, h₂⟩ := h₂
-  rw [List.mem_iff_getElem] at h₂
-  replace ⟨i, h, h₂⟩ := h₂
-  have ⟨u, v, h₄⟩ : ∃ u v, w = u ++ [.nonterminal 𝔡] ++ v := by
-    use w.take i
-    use w.drop (i + 1)
-    rw [← h₂]
-    simp only [List.take_append_getElem, List.take_append_drop]
-  subst h₄
-  replace ⟨𝔡', h₁', h₁⟩  := h₁ 𝔡 h₃ t
-  use 𝔡', h₁'
-  simp only [EDT0LGrammar.rewriteWord_append]
-  conv =>
-    arg 1; arg 1; arg 2
-    simp only [rewriteWord_cons, rewriteSymbol_nonterminal, rewriteWord_nil,
-      List.append_nil]
-  simp_all only [
-    List.append_assoc, List.cons_append, List.nil_append, List.mem_append, true_or, or_true]
+lemma isDeadEndSingleton_iff_isDeadEndSet {α V T} {E : EDT0LGrammar α V T} {𝔡 : V} :
+    E.IsDeadEndSingleton 𝔡 ↔ E.IsDeadEndSet {𝔡} := by rfl
 
-lemma rewrites_dead_end (w w' : List (Symbol α V)) (dead : Finset V)
-  (h₁ : E.HasDeadEnds dead)
-  (h₂ : ∃ 𝔡 ∈ dead, .nonterminal 𝔡 ∈ w)
-  (h₃ : E.rewrites w w') :
-    ∃ 𝔡' ∈ dead, .nonterminal 𝔡' ∈ w' := by
-  unfold rewrites at h₃
-  replace ⟨τ, h₃⟩ := h₃
-  subst h₃
-  exact rewrite_word_dead_end E w τ dead h₁ h₂
+lemma isDeadEndSingleton_iff {α V T} (E : EDT0LGrammar α V T) (𝔡 : V) :
+    E.IsDeadEndSingleton 𝔡 ↔ ∀ t : T, .nonterminal 𝔡 ∈ E.table t 𝔡 := by
+  unfold IsDeadEndSingleton IsDeadEndSet
+  simp
 
-lemma derives_dead_end (w w' : List (Symbol α V)) (dead : Finset V)
-  (h₁ : E.HasDeadEnds dead)
-  (h₂ : ∃ 𝔡 ∈ dead, .nonterminal 𝔡 ∈ w)
-  (h₃ : E.derives w w') :
-    ∃ 𝔡' ∈ dead, .nonterminal 𝔡' ∈ w' := by
-  induction h₃ with
+lemma rewriteWord_dead_word {α V T} (E : EDT0LGrammar α V T) (w : List (Symbol α V))
+  (h : E.IsDeadWord w) (t : T) :
+    E.IsDeadWord (E.rewriteWord t w) := by
+  replace ⟨dead, h, 𝔡, h', h''⟩ := h
+  use dead, h
+  rw [List.mem_iff_append] at h''
+  obtain ⟨u, v, rfl⟩ := h''
+  simp only [rewriteWord_append, rewriteWord_cons, rewriteSymbol_nonterminal, List.mem_append,
+    exists_prop]
+  replace ⟨𝔡', h𝔡', h⟩ := h 𝔡 h' t
+  use 𝔡', h𝔡'
+  right; left
+  exact h
+
+lemma rewrites_dead_word {α V T} (E : EDT0LGrammar α V T) (u v : List (Symbol α V))
+  (h_u : E.IsDeadWord u) (h_rewrites : E.Rewrites u v) :
+    E.IsDeadWord v := by
+  obtain ⟨t, rfl⟩ := h_rewrites
+  exact rewriteWord_dead_word E u h_u t
+
+lemma derives_dead_word {α V T} (E : EDT0LGrammar α V T) (u v : List (Symbol α V))
+  (h_u : E.IsDeadWord u) (h_derives : E.Derives u v) :
+    E.IsDeadWord v := by
+  induction h_derives with
   | refl =>
-    exact h₂
-  | tail ih₁ ih₂ ih₃ =>
-    rename_i x y
-    exact rewrites_dead_end E x y dead h₁ ih₃ ih₂
-
-lemma rewrite_dead_word (w : List (Symbol α V)) (t : T) (h : E.DeadWord w) :
-    E.DeadWord (E.rewriteWord t w) := by
-  replace ⟨𝔇, h, h'⟩ := h
-  use 𝔇, h
-  exact E.rewrite_word_dead_end w t 𝔇 h h'
-
-lemma rewrites_dead_word (w w' : List (Symbol α V)) (h : E.DeadWord w) (h' : E.rewrites w w') :
-    E.DeadWord w' := by
-  replace ⟨𝔇, h₁, h⟩ := h
-  use 𝔇, h₁
-  exact rewrites_dead_end E w w' 𝔇 h₁ h h'
-
-lemma derives_dead_word (w w' : List (Symbol α V)) (h : E.DeadWord w) (h' : E.derives w w') :
-    E.DeadWord w' := by
-  --
-  replace ⟨𝔇, h₁, h⟩ := h
-  use 𝔇, h₁
-  exact derives_dead_end E w w' 𝔇 h₁ h h'
-
-lemma derives_from_dead_word (w : List (Symbol α V)) (h : E.DeadWord w) :
-    ∀ w' : List α, ¬(E.derives w (w'.map .terminal)) := by
-  intro w' h'
-  replace h' := E.derives_dead_word _ _ h h'
-  replace ⟨_, _, 𝔡, _, h''⟩ := h'
-  simp_all only [List.mem_iff_getElem,List.getElem_map, reduceCtorEq, List.length_map, exists_false]
+    exact h_u
+  | tail x y h =>
+    rename_i a b
+    exact rewrites_dead_word E a b h y
 
 end EDT0LGrammar
