LSystems/EDT0L/Union.lean
@@ -3,942 +3,317 @@ Copyright (c) 2025 Alex Bishop. All rights reserved.
 Released under Apache 2.0 license as described in the file LICENSE.
 Author: Alex Bishop
 -/
-import LSystems.EDT0L.Defs
+module
+
+public import LSystems.EDT0L.Defs
+
+/-!
+# EDT0L languages are closed under union
+
+This file provides a constructive proof that the family of EDT0L languages is closed under taking
+unions.
+
+## Main definition
+
+* `EDT0LGrammar.Union E_l E_r`: an EDT0L grammar whose language is the union of the languages of
+  `E_l` and `E_r`.
+
+## Main theorem
+
+* `EDT0LGrammar.Union.defines_union`: the above definition does precicely what is expected.
+* `Language.isEDT0L_union`: the union of two EDT0L languages is EDT0l.
+-/
+
+@[expose] public section
 
 namespace EDT0LGrammar
-variable {α V₀ T₀ V₁ T₁ : Type*} [Fintype V₀] [Fintype T₀] [Fintype V₁] [Fintype T₁]
+inductive Union.extended_nonterminals (V₀ V₁ : Type*) where
+  | lhs (v : V₀)
+  | rhs (v : V₁)
+  | init
+deriving Fintype, DecidableEq
 
-structure UnionData where
-  E₀ : EDT0LGrammar α V₀ T₀
-  E₁ : EDT0LGrammar α V₁ T₁
+inductive Union.extended_tables (T₀ T₁ : Type*) where
+  | lhs (v : T₀)
+  | rhs (v : T₁)
+  | init_lhs
+  | init_rhs
+deriving Fintype, DecidableEq
 
-namespace UnionData
-variable (data : @UnionData α V₀ T₀ V₁ T₁ _ _ _ _)
+abbrev Union.map_symbol_lhs {α V₀ V₁ : Type*} : Symbol α V₀ → Symbol α (extended_nonterminals V₀ V₁)
+  | .terminal t => .terminal t
+  | .nonterminal n => .nonterminal (.lhs n)
 
-def extend_alphabet₀ : Symbol α V₀ → Symbol α ((V₀ ⊕ V₁) ⊕ Unit)
-  | .terminal a => .terminal a
-  | .nonterminal v => .nonterminal (.inl (.inl v))
+abbrev Union.map_symbol_rhs {α V₀ V₁ : Type*} : Symbol α V₁ → Symbol α (extended_nonterminals V₀ V₁)
+  | .terminal t => .terminal t
+  | .nonterminal n => .nonterminal (.rhs n)
 
-def extend_alphabet₁ : Symbol α V₁ → Symbol α ((V₀ ⊕ V₁) ⊕ Unit)
-  | .terminal a => .terminal a
-  | .nonterminal v => .nonterminal (.inl (.inr v))
+variable {α V₀ T₀ V₁ T₁ : Type*} (E₀ : EDT0LGrammar α V₀ T₀) (E₁ : EDT0LGrammar α V₁ T₁) in
+def Union : EDT0LGrammar α (Union.extended_nonterminals V₀ V₁) (Union.extended_tables T₀ T₁) where
+  initial := .init
+  table := fun
+    | .lhs t₀, .lhs v₀ => List.map Union.map_symbol_lhs (E₀.table t₀ v₀)
+    | .rhs t₁, .rhs v₁ => List.map Union.map_symbol_rhs (E₁.table t₁ v₁) 
+    | .init_lhs, .init => [ .nonterminal <| .lhs E₀.initial ]
+    | .init_rhs, .init => [ .nonterminal <| .rhs E₁.initial ] 
+    | _, v => [.nonterminal v]
 
-section extend_alphabets
-variable {α V₀ V₁ : Type*}
-
+variable {α V₀ T₀ V₁ T₁ : Type*} (E₀ : EDT0LGrammar α V₀ T₀) (E₁ : EDT0LGrammar α V₁ T₁) in
 @[simp]
-lemma extend_alphabet₀_terminal {a : α} :
-    @extend_alphabet₀ α V₀ V₁ (.terminal a) = (.terminal a) := rfl
-
-@[simp]
-lemma extend_alphabet₁_terminal {a : α} :
-    @extend_alphabet₁ α V₀ V₁ (.terminal a) = (.terminal a) := rfl
-
-@[simp]
-lemma extend_alphabet₀_nonterminal {v : V₀} :
-    @extend_alphabet₀ α V₀ V₁ (.nonterminal v) = (.nonterminal <| .inl <| .inl <| v) := rfl
-
-@[simp]
-lemma extend_alphabet₁_nonterminal {v : V₁} :
-    @extend_alphabet₁ α V₀ V₁ (.nonterminal v) = (.nonterminal <| .inl <| .inr <| v) := rfl
-
-@[simp]
-lemma extend_alphabet₀_terminal_word {w : List α} :
-    List.map (@extend_alphabet₀ α V₀ V₁) (List.map .terminal w)
-    = List.map .terminal w := by
-  --
-  induction w with
-  | nil =>
-    simp only [List.map_nil]
-  | cons a as ih =>
-    simp_all only [
-      List.map_map, List.map_inj_left,
-      Function.comp_apply, List.map_cons, List.cons.injEq, implies_true,
-      and_true]
-    rfl
-
-@[simp]
-lemma extend_alphabet₁_terminal_word (w : List α) :
-    List.map (@extend_alphabet₁ α V₀ V₁) (List.map .terminal w)
-    = List.map .terminal w := by
-  --
-  induction w with
-  | nil =>
-    simp only [List.map_nil]
-  | cons a as ih =>
-    simp_all only [
-      List.map_map, List.map_inj_left,
-      Function.comp_apply, List.map_cons, List.cons.injEq, implies_true,
-      and_true]
-    rfl
-
-end extend_alphabets
-
-def grammar : EDT0LGrammar α ((V₀ ⊕ V₁) ⊕ Unit) ((T₀ ⊕ T₁) ⊕ Fin 2) where
-  initial := .inr ()
-  tables := fun h n ↦ match h with
-    | .inl (.inl τ₀) => match n with
-      | .inl (.inl n₀) => (data.E₀.tables τ₀ n₀).map extend_alphabet₀
-      | _ => [.nonterminal n]
-    | .inl (.inr τ₁) => match n with
-      | .inl (.inr n₁) => (data.E₁.tables τ₁ n₁).map extend_alphabet₁
-      | _ => [.nonterminal n]
-    | .inr 0 => match n with
-      | .inl s => [.nonterminal (.inl s)]
-      | .inr _ => [.nonterminal (.inl (.inl data.E₀.initial))]
-    | .inr 1 => match n with
-      | .inl s => [.nonterminal (.inl s)]
-      | .inr _ => [.nonterminal (.inl (.inr data.E₁.initial))]
-
-lemma left_rewrites (w : List (Symbol α ((V₀ ⊕ V₁) ⊕ Unit)))
-  (w' : List (Symbol α ((V₀ ⊕ V₁) ⊕ Unit)))
-  (h : ∃ u : List (Symbol α V₀), w = u.map extend_alphabet₀ ∧ data.E₀.generates u) :
-    data.grammar.rewrites w w'
-      → ∃ u' : List (Symbol α V₀), w' = u'.map extend_alphabet₀ ∧ data.E₀.generates u' := by
-  --
-  intro h₁
-  have ⟨u, ⟨h_l, h_r⟩⟩ := h
-  clear h
-  unfold EDT0LGrammar.rewrites at h₁
-  unfold EDT0LGrammar.rewriteWord at h₁
-  unfold EDT0LGrammar.rewriteSymbol at h₁
-  unfold UnionData.grammar at h₁
-  unfold extend_alphabet₀ at h_l
-  simp only at h₁
-  subst h_l
-  replace ⟨τ, h₁⟩ := h₁
-  simp [List.flatMap_map] at h₁
-  match τ with
-  | .inl (.inl τ₀) =>
-      simp only at h₁
-      change
-        let inner := _;
-        @List.flatMap _ _ inner _ = _
-        at h₁
-      extract_lets inner at h₁
-      have hh : inner = fun a ↦ List.map extend_alphabet₀ (data.E₀.rewriteSymbol τ₀ a) := by
-        unfold extend_alphabet₀
-        unfold inner
-        funext a
-        subst h₁
-        clear τ
-        split
-        · rename_i x t heq
-          split at heq
-          · rename_i x_1 t_1
-            simp_all only [Symbol.terminal.injEq]
-            subst heq
-            rfl
-          · rename_i x_1 n
-            simp_all only [reduceCtorEq]
-        · rename_i x n heq
-          cases n with
-          | inl val =>
-            cases val with
-            | inl val_1 =>
-              simp_all only
-              split at heq
-              next x_1 t => simp_all only [reduceCtorEq]
-              next x_1 n =>
-                simp_all only [Symbol.nonterminal.injEq, Sum.inl.injEq]
-                subst heq
-                rfl
-            | inr val_2 =>
-              simp_all only
-              split at heq
-              next x_1 t => simp_all only [reduceCtorEq]
-              next x_1 n => simp_all only [Symbol.nonterminal.injEq, Sum.inl.injEq, reduceCtorEq]
-          | inr val_1 =>
-            simp_all only
-            split at heq
-            next x_1 t => simp_all only [reduceCtorEq]
-            next x_1 n => simp_all only [Symbol.nonterminal.injEq, reduceCtorEq]
-      rw [hh] at h₁
-      clear hh
-      clear inner
-
-      rw [← List.flatMap_map] at h₁
-      rw [← List.map_flatMap] at h₁
-      change
-        let u' := _;
-        List.map extend_alphabet₀ u' = _
-        at h₁
-      extract_lets u' at h₁
-      use u'
-      constructor
-      · exact Eq.symm h₁
-      · have hh : data.E₀.rewrites u u' := by
-          use τ₀
-          unfold rewriteWord
-          subst u'
-          rw [List.flatMap_id', ← List.flatMap_def]
-        unfold EDT0LGrammar.generates
-        unfold EDT0LGrammar.generates at h_r
-        unfold EDT0LGrammar.derives
-        unfold EDT0LGrammar.derives at h_r
-        exact Relation.ReflTransGen.tail h_r hh
-  | .inl (.inr τ₁) =>
-    simp only at h₁
-    change
-      let inner := _;
-      @List.flatMap _ _ inner _ = _
-      at h₁
-    extract_lets inner at h₁
-    have hh : inner = fun a ↦ [extend_alphabet₀ a] := by
-      unfold inner
-      funext a
-      clear h₁
-      clear inner
-      clear τ
-      -- aesop
-      split
-      next x t heq =>
-        simp_all only [List.cons.injEq, and_true]
-        split at heq
-        next x_1 t_1 =>
-          simp_all only [Symbol.terminal.injEq]
-          subst heq
-          rfl
-        next x_1 n => simp_all only [reduceCtorEq]
-      next x n heq =>
-        cases n with
-        | inl val =>
-          cases val with
-          | inl val_1 =>
-            simp_all only [List.cons.injEq, and_true]
-            split at heq
-            next x_1 t => simp_all only [reduceCtorEq]
-            next x_1 n =>
-              simp_all only [Symbol.nonterminal.injEq, Sum.inl.injEq]
-              subst heq
-              rfl
-          | inr val_2 =>
-            simp_all only [List.map_eq_singleton_iff]
-            split at heq
-            next x_1 t => simp_all only [reduceCtorEq]
-            next x_1 n => simp_all only [Symbol.nonterminal.injEq, Sum.inl.injEq, reduceCtorEq]
-        | inr val_1 =>
-          simp_all only [List.cons.injEq, and_true]
-          split at heq
-          next x_1 t => simp_all only [reduceCtorEq]
-          next x_1 n => simp_all only [Symbol.nonterminal.injEq, reduceCtorEq]
-    use u
-    rw [← h₁, hh]
-    constructor
-    · rw [← List.map_eq_flatMap]
-    · exact h_r
-  | .inr 0 =>
-    simp only at h₁
-    change
-      let inner := _;
-      @List.flatMap _ _ inner _ = _
-      at h₁
-    extract_lets inner at h₁
-    have hh : inner = fun a ↦ [extend_alphabet₀ a] := by
-      unfold inner
-      funext a
-      clear h₁
-      clear inner
-      clear τ
-      -- aesop
-      split
-      next x t heq =>
-        simp_all only [List.cons.injEq, and_true]
-        split at heq
-        next x_1 t_1 =>
-          simp_all only [Symbol.terminal.injEq]
-          subst heq
-          rfl
-        next x_1 n => simp_all only [reduceCtorEq]
-      next x n heq =>
-        cases n with
-        | inl val =>
-          cases val with
-          | inl val_1 =>
-            simp_all only [List.cons.injEq, and_true]
-            split at heq
-            next x_1 t => simp_all only [reduceCtorEq]
-            next x_1 n =>
-              simp_all only [Symbol.nonterminal.injEq, Sum.inl.injEq]
-              subst heq
-              rfl
-          | inr val_2 =>
-            split at heq
-            next x_1 t => simp_all only [reduceCtorEq]
-            next x_1 n => simp_all only [Symbol.nonterminal.injEq, Sum.inl.injEq, reduceCtorEq]
-        | inr val_1 =>
-          simp_all only [List.cons.injEq, and_true]
-          split at heq
-          next x_1 t => simp_all only [reduceCtorEq]
-          next x_1 n => simp_all only [Symbol.nonterminal.injEq, reduceCtorEq]
-    use u
-    rw [← h₁, hh]
-    constructor
-    · rw [← List.map_eq_flatMap]
-    · exact h_r
-  | .inr 1 =>
-    simp only at h₁
-    change
-      let inner := _;
-      @List.flatMap _ _ inner _ = _
-      at h₁
-    extract_lets inner at h₁
-    have hh : inner = fun a ↦ [extend_alphabet₀ a] := by
-      unfold inner
-      funext a
-      clear h₁
-      clear inner
-      clear τ
-      -- aesop
-      split
-      next x t heq =>
-        simp_all only [List.cons.injEq, and_true]
-        split at heq
-        next x_1 t_1 =>
-          simp_all only [Symbol.terminal.injEq]
-          subst heq
-          rfl
-        next x_1 n => simp_all only [reduceCtorEq]
-      next x n heq =>
-        cases n with
-        | inl val =>
-          cases val with
-          | inl val_1 =>
-            simp_all only [List.cons.injEq, and_true]
-            split at heq
-            next x_1 t => simp_all only [reduceCtorEq]
-            next x_1 n =>
-              simp_all only [Symbol.nonterminal.injEq, Sum.inl.injEq]
-              subst heq
-              rfl
-          | inr val_2 =>
-            split at heq
-            next x_1 t => simp_all only [reduceCtorEq]
-            next x_1 n => simp_all only [Symbol.nonterminal.injEq, Sum.inl.injEq, reduceCtorEq]
-        | inr val_1 =>
-          simp_all only [List.cons.injEq, and_true]
-          split at heq
-          next x_1 t => simp_all only [reduceCtorEq]
-          next x_1 n => simp_all only [Symbol.nonterminal.injEq, reduceCtorEq]
-    use u
-    rw [← h₁, hh]
-    constructor
-    · rw [← List.map_eq_flatMap]
-    · exact h_r
-
-lemma right_rewrites (w : List (Symbol α ((V₀ ⊕ V₁) ⊕ Unit)))
-  (w' : List (Symbol α ((V₀ ⊕ V₁) ⊕ Unit)))
-  (h : ∃ u : List (Symbol α V₁), w = u.map extend_alphabet₁ ∧ data.E₁.generates u) :
-    data.grammar.rewrites w w'
-      → ∃ u' : List (Symbol α V₁), w' = u'.map extend_alphabet₁ ∧ data.E₁.generates u' := by
-  intro h₁
-  have ⟨u, ⟨h_l, h_r⟩⟩ := h
-  clear h
-  unfold EDT0LGrammar.rewrites at h₁
-  unfold EDT0LGrammar.rewriteWord at h₁
-  unfold EDT0LGrammar.rewriteSymbol at h₁
-  unfold UnionData.grammar at h₁
-  unfold extend_alphabet₁ at h_l
-  simp only at h₁
-  subst h_l
-  replace ⟨τ, h₁⟩ := h₁
-  simp [List.flatMap_map] at h₁
-  match τ with
-  | .inl (.inr τ₁) =>
-      simp only at h₁
-      change
-        let inner := _;
-        @List.flatMap _ _ inner _ = _
-        at h₁
-      extract_lets inner at h₁
-      have hh : inner = fun a ↦ List.map extend_alphabet₁ (data.E₁.rewriteSymbol τ₁ a) := by
-        unfold extend_alphabet₁
-        unfold inner
-        funext a
-        subst h₁
-        clear τ
-        --FIXME aesop?
-        split
-        next x t heq =>
-          split at heq
-          next x_1 t_1 =>
-            simp_all only [Symbol.terminal.injEq]
-            subst heq
-            rfl
-          next x_1 n => simp_all only [reduceCtorEq]
-        next x n heq =>
-          cases n with
-          | inl val =>
-            cases val with
-            | inl val_1 =>
-              simp_all only
-              split at heq
-              next x_1 t => simp_all only [reduceCtorEq]
-              next x_1 n => simp_all only [Symbol.nonterminal.injEq, Sum.inl.injEq, reduceCtorEq]
-            | inr val_2 =>
-              simp_all only
-              split at heq
-              next x_1 t => simp_all only [reduceCtorEq]
-              next x_1 n =>
-                simp_all only [Symbol.nonterminal.injEq, Sum.inl.injEq, Sum.inr.injEq]
-                subst heq
-                rfl
-          | inr val_1 =>
-            simp_all only
-            split at heq
-            next x_1 t => simp_all only [reduceCtorEq]
-            next x_1 n => simp_all only [Symbol.nonterminal.injEq, reduceCtorEq]
-      rw [hh] at h₁
-      clear hh
-      clear inner
-
-      rw [← List.flatMap_map] at h₁
-      rw [← List.map_flatMap] at h₁
-      change
-        let u' := _;
-        List.map extend_alphabet₁ u' = _
-        at h₁
-      extract_lets u' at h₁
-      use u'
-      constructor
-      · exact Eq.symm h₁
-      · have hh : data.E₁.rewrites u u' := by
-          use τ₁
-          unfold rewriteWord
-          subst u'
-          rw [List.flatMap_id', ← List.flatMap_def]
-        unfold EDT0LGrammar.generates
-        unfold EDT0LGrammar.generates at h_r
-        unfold EDT0LGrammar.derives
-        unfold EDT0LGrammar.derives at h_r
-        exact Relation.ReflTransGen.tail h_r hh
-  | .inl (.inl τ₀) =>
-    simp only at h₁
-    change
-      let inner := _;
-      @List.flatMap _ _ inner _ = _
-      at h₁
-    extract_lets inner at h₁
-    have hh : inner = fun a ↦ [extend_alphabet₁ a] := by
-      unfold inner
-      funext a
-      clear h₁
-      clear inner
-      clear τ
-      -- aesop
-      split
-      next x t heq =>
-        simp_all only [List.cons.injEq, and_true]
-        split at heq
-        next x_1 t_1 =>
-          simp_all only [Symbol.terminal.injEq]
-          subst heq
-          rfl
-        next x_1 n => simp_all only [reduceCtorEq]
-      next x n heq =>
-        cases n with
-        | inl val =>
-          cases val with
-          | inl val_1 =>
-            simp_all only [List.map_eq_singleton_iff]
-            split at heq
-            next x_1 t => simp_all only [reduceCtorEq]
-            next x_1 n => simp_all only [Symbol.nonterminal.injEq, Sum.inl.injEq, reduceCtorEq]
-          | inr val_2 =>
-            simp_all only [List.cons.injEq, and_true]
-            split at heq
-            next x_1 t => simp_all only [reduceCtorEq]
-            next x_1 n =>
-              simp_all only [Symbol.nonterminal.injEq, Sum.inl.injEq, Sum.inr.injEq]
-              subst heq
-              rfl
-        | inr val_1 =>
-          simp_all only [List.cons.injEq, and_true]
-          split at heq
-          next x_1 t => simp_all only [reduceCtorEq]
-          next x_1 n => simp_all only [Symbol.nonterminal.injEq, reduceCtorEq]
-    use u
-    rw [← h₁, hh]
-    constructor
-    · rw [← List.map_eq_flatMap]
-    · exact h_r
-  | .inr 0 =>
-    simp only at h₁
-    change
-      let inner := _;
-      @List.flatMap _ _ inner _ = _
-      at h₁
-    extract_lets inner at h₁
-    have hh : inner = fun a ↦ [extend_alphabet₁ a] := by
-      unfold inner
-      funext a
-      clear h₁
-      clear inner
-      clear τ
-      -- aesop
-      split
-      next x t heq =>
-        simp_all only [List.cons.injEq, and_true]
-        split at heq
-        next x_1 t_1 =>
-          simp_all only [Symbol.terminal.injEq]
-          subst heq
-          rfl
-        next x_1 n => simp_all only [reduceCtorEq]
-      next x n heq =>
-        cases n with
-        | inl val =>
-          cases val with
-          | inl val_1 =>
-            simp_all only [List.cons.injEq, and_true]
-            split at heq
-            next x_1 t => simp_all only [reduceCtorEq]
-            next x_1 n => simp_all only [Symbol.nonterminal.injEq, Sum.inl.injEq, reduceCtorEq]
-          | inr val_2 =>
-            simp_all only [List.cons.injEq, and_true]
-            split at heq
-            next x_1 t => simp_all only [reduceCtorEq]
-            next x_1 n =>
-              simp_all only [Symbol.nonterminal.injEq, Sum.inl.injEq, Sum.inr.injEq]
-              subst heq
-              rfl
-        | inr val_1 =>
-          simp_all only [List.cons.injEq, and_true]
-          split at heq
-          next x_1 t => simp_all only [reduceCtorEq]
-          next x_1 n => simp_all only [Symbol.nonterminal.injEq, reduceCtorEq]
-    use u
-    rw [← h₁, hh]
-    constructor
-    · rw [← List.map_eq_flatMap]
-    · exact h_r
-  | .inr 1 =>
-    simp only at h₁
-    change
-      let inner := _;
-      @List.flatMap _ _ inner _ = _
-      at h₁
-    extract_lets inner at h₁
-    have hh : inner = fun a ↦ [extend_alphabet₁ a] := by
-      unfold inner
-      funext a
-      clear h₁
-      clear inner
-      clear τ
-      -- aesop
-      split
-      next x t heq =>
-        simp_all only [List.cons.injEq, and_true]
-        split at heq
-        next x_1 t_1 =>
-          simp_all only [Symbol.terminal.injEq]
-          subst heq
-          rfl
-        next x_1 n => simp_all only [reduceCtorEq]
-      next x n heq =>
-        cases n with
-        | inl val =>
-          cases val with
-          | inl val_1 =>
-            simp_all only [List.cons.injEq, and_true]
-            split at heq
-            next x_1 t => simp_all only [reduceCtorEq]
-            next x_1 n => simp_all only [Symbol.nonterminal.injEq, Sum.inl.injEq, reduceCtorEq]
-          | inr val_2 =>
-            simp_all only [List.cons.injEq, and_true]
-            split at heq
-            next x_1 t => simp_all only [reduceCtorEq]
-            next x_1 n =>
-              simp_all only [Symbol.nonterminal.injEq, Sum.inl.injEq, Sum.inr.injEq]
-              subst heq
-              rfl
-        | inr val_1 =>
-          simp_all only [List.cons.injEq, and_true]
-          split at heq
-          next x_1 t => simp_all only [reduceCtorEq]
-          next x_1 n => simp_all only [Symbol.nonterminal.injEq, reduceCtorEq]
-    use u
-    rw [← h₁, hh]
-    constructor
-    · rw [← List.map_eq_flatMap]
-    · exact h_r
-
-lemma basic_property
-  (w : List (Symbol α ((V₀ ⊕ V₁) ⊕ Unit)))
-  (h : data.grammar.generates w) :
-    w = [.nonterminal data.grammar.initial]
-    ∨ (∃ u : List (Symbol α V₀), w = u.map extend_alphabet₀ ∧ data.E₀.generates u)
-    ∨ (∃ u : List (Symbol α V₁), w = u.map extend_alphabet₁ ∧ data.E₁.generates u) := by
-  --
-  induction h
-  case refl => left; rfl
-  case tail a b ih₁ ih₂ ih₃ =>
-    cases ih₃
-    · rename_i ih₃
-      -- we are rewriting the starting symbol
-      replace ⟨τ, ih₂⟩ := ih₂
-      match τ with
-      | .inl (.inl τ₀) =>
-        left
-        rw [← ih₂, ih₃]
-        unfold EDT0LGrammar.rewriteWord
-        unfold EDT0LGrammar.rewriteSymbol
-        unfold UnionData.grammar
-        simp only
-        rw [List.flatMap_cons, List.flatMap_nil, List.append_nil]
-      | .inl (.inr τ₁) =>
-        left
-        rw [← ih₂, ih₃]
-        unfold EDT0LGrammar.rewriteWord
-        unfold EDT0LGrammar.rewriteSymbol
-        unfold UnionData.grammar
-        simp only
-        rw [List.flatMap_cons, List.flatMap_nil, List.append_nil]
-      | .inr 0 =>
-        right ; left
-        use [.nonterminal data.E₀.initial]
-        constructor
-        · rw [← ih₂, ih₃]
-          unfold extend_alphabet₀
-          unfold EDT0LGrammar.rewriteWord
-          unfold EDT0LGrammar.rewriteSymbol
-          unfold UnionData.grammar
-          simp only
-          rw [List.map_cons, List.map_nil, List.flatMap_cons, List.flatMap_nil, List.append_nil]
-        · unfold EDT0LGrammar.generates
-          unfold EDT0LGrammar.derives
-          exact Relation.ReflTransGen.refl
-      | .inr 1 =>
-        right ; right
-        use [.nonterminal data.E₁.initial]
-        constructor
-        · rw [← ih₂, ih₃]
-          unfold extend_alphabet₁
-          unfold EDT0LGrammar.rewriteWord
-          unfold EDT0LGrammar.rewriteSymbol
-          unfold UnionData.grammar
-          simp only
-          rw [List.map_cons, List.map_nil, List.flatMap_cons, List.flatMap_nil, List.append_nil]
-        · unfold EDT0LGrammar.generates
-          unfold EDT0LGrammar.derives
-          exact Relation.ReflTransGen.refl
-    · rename_i ih₃
-      cases ih₃
-      · rename_i ih₃
-        right; left
-        exact data.left_rewrites a b ih₃ ih₂
-      · rename_i ih₃
-        right; right
-        exact data.right_rewrites a b ih₃ ih₂
-
-lemma basic_property₀
-  (w : List (Symbol α V₀))
-  (h : data.E₀.generates w) :
-    data.grammar.generates (w.map extend_alphabet₀) := by
-  --
-  induction h
-  case refl =>
-    unfold EDT0LGrammar.generates
-    unfold EDT0LGrammar.derives
-    apply Relation.ReflTransGen.tail (Relation.ReflTransGen.refl) ?_
-    unfold EDT0LGrammar.rewrites
-    use .inr 0
-    unfold EDT0LGrammar.rewriteWord
-    unfold EDT0LGrammar.rewriteSymbol
-    unfold UnionData.grammar
+lemma Union.rewriteSymbol_lhs (t s) :
+    (Union E₀ E₁).rewriteSymbol t (Union.map_symbol_lhs s) =
+      match t with
+      | .lhs t' =>
+        List.map Union.map_symbol_lhs (E₀.rewriteSymbol t' s)
+      | .rhs _ | .init_lhs | .init_rhs =>
+        [Union.map_symbol_lhs s]
+    := by
+  match t with
+  | .lhs t' =>
+    unfold Union rewriteSymbol
     simp only
-    unfold extend_alphabet₀
-    simp only [List.flatMap_cons, List.flatMap_nil, List.append_nil, List.map_cons, List.map_nil]
-  case tail x y z ih₁ ih₂ =>
-    have hh :
-        data.grammar.rewrites
-          (List.map extend_alphabet₀ x)
-          (List.map extend_alphabet₀ y) := by
-      have ⟨ τ, h ⟩ := ih₁
-      rw [← h]
-      use .inl (.inl τ)
-      unfold EDT0LGrammar.rewriteWord
-      unfold EDT0LGrammar.rewriteSymbol
-      unfold UnionData.grammar
-      --
-      unfold extend_alphabet₀
+    match s with
+    | .terminal _ =>
+      simp only [List.map_cons, List.map_nil]
+    | .nonterminal _ =>
       simp only
-      simp only [List.flatMap_map, List.map_flatMap]
-      clear h
-      clear z
-      change
-        let f_l := List.flatMap _;
-        let f_r := List.flatMap _;
-        f_l x = f_r x
-      extract_lets f_l f_r
-      have hh : f_l = f_r := by
-        unfold f_l
-        unfold f_r
-        funext xx
-        induction xx
-        · simp only [List.flatMap_nil]
-        · rename_i a as ih
-          -- aesop
-          simp_all only [List.flatMap_cons, List.append_cancel_right_eq]
-          split
-          next x_1 t heq =>
-            split
-            next x_2 t_1 => simp_all only [Symbol.terminal.injEq, List.map_cons, List.map_nil]
-            next x_2 n => simp_all only [reduceCtorEq]
-          next x_1 n heq =>
-            cases n with
-            | inl val =>
-              cases val with
-              | inl val_1 =>
-                simp_all only
-                split
-                next x_2 t => simp_all only [reduceCtorEq]
-                next x_2 n => simp_all only [Symbol.nonterminal.injEq, Sum.inl.injEq]
-              | inr val_2 =>
-                simp_all only
-                split
-                next x_2 t => simp_all only [reduceCtorEq]
-                next x_2 n => simp_all only [Symbol.nonterminal.injEq, Sum.inl.injEq, reduceCtorEq]
-            | inr val_1 =>
-              simp_all only
-              split
-              next x_2 t => simp_all only [reduceCtorEq]
-              next x_2 n => simp_all only [Symbol.nonterminal.injEq, reduceCtorEq]
-      rw [hh]
-    unfold EDT0LGrammar.generates
-    unfold EDT0LGrammar.generates at ih₂
-    unfold EDT0LGrammar.derives
-    unfold EDT0LGrammar.derives at ih₂
-    exact Relation.ReflTransGen.tail ih₂ hh
-
-lemma basic_property₁
-  (w : List (Symbol α V₁))
-  (h : data.E₁.generates w) :
-    data.grammar.generates (w.map extend_alphabet₁) := by
-  --
-  induction h
-  case refl =>
-    unfold EDT0LGrammar.generates
-    unfold EDT0LGrammar.derives
-    apply Relation.ReflTransGen.tail (Relation.ReflTransGen.refl) ?_
-    unfold EDT0LGrammar.rewrites
-    use .inr 1
-    unfold EDT0LGrammar.rewriteWord
-    unfold EDT0LGrammar.rewriteSymbol
-    unfold UnionData.grammar
+  | .rhs _ | .init_lhs | .init_rhs =>
+    unfold Union rewriteSymbol
     simp only
-    unfold extend_alphabet₁
-    simp only [List.flatMap_cons, List.flatMap_nil, List.append_nil, List.map_cons, List.map_nil]
-  case tail x y z ih₁ ih₂ =>
-    have hh :
-        data.grammar.rewrites
-          (List.map extend_alphabet₁ x)
-          (List.map extend_alphabet₁ y) := by
-      have ⟨ τ, h ⟩ := ih₁
-      rw [← h]
-      use .inl (.inr τ)
-      unfold EDT0LGrammar.rewriteWord
-      unfold EDT0LGrammar.rewriteSymbol
-      unfold UnionData.grammar
-      --
-      unfold extend_alphabet₁
+    match s with | .terminal _ | .nonterminal _ => simp only
+
+variable {α V₀ T₀ V₁ T₁ : Type*} (E₀ : EDT0LGrammar α V₀ T₀) (E₁ : EDT0LGrammar α V₁ T₁) in
+@[simp]
+lemma Union.rewriteSymbol_rhs (t s) :
+    (Union E₀ E₁).rewriteSymbol t (Union.map_symbol_rhs s) =
+      match t with
+      | .rhs t' =>
+        List.map Union.map_symbol_rhs (E₁.rewriteSymbol t' s)
+      | .lhs _ | .init_lhs | .init_rhs =>
+        [Union.map_symbol_rhs s]
+    := by
+  match t with
+  | .rhs t' =>
+    unfold Union rewriteSymbol
+    simp only
+    match s with
+    | .terminal _ =>
+      simp only [List.map_cons, List.map_nil]
+    | .nonterminal _ =>
       simp only
-      simp only [List.flatMap_map, List.map_flatMap]
-      clear h
-      clear z
-      change
-        let f_l := List.flatMap _;
-        let f_r := List.flatMap _;
-        f_l x = f_r x
-      extract_lets f_l f_r
-      have hh : f_l = f_r := by
-        unfold f_l
-        unfold f_r
-        funext xx
-        induction xx
-        · simp only [List.flatMap_nil]
-        · rename_i a as ih
-          -- aesop
-          simp_all only [List.flatMap_cons, List.append_cancel_right_eq]
-          split
-          next x_1 t heq =>
-            split
-            next x_2 t_1 => simp_all only [Symbol.terminal.injEq, List.map_cons, List.map_nil]
-            next x_2 n => simp_all only [reduceCtorEq]
-          next x_1 n heq =>
-            cases n with
-            | inl val =>
-              cases val with
-              | inl val_1 =>
-                simp_all only
-                split
-                next x_2 t => simp_all only [reduceCtorEq]
-                next x_2 n => simp_all only [Symbol.nonterminal.injEq, Sum.inl.injEq, reduceCtorEq]
-              | inr val_2 =>
-                simp_all only
-                split
-                next x_2 t => simp_all only [reduceCtorEq]
-                next x_2 n => simp_all only [Symbol.nonterminal.injEq, Sum.inl.injEq, Sum.inr.injEq]
-            | inr val_1 =>
-              simp_all only
-              split
-              next x_2 t => simp_all only [reduceCtorEq]
-              next x_2 n => simp_all only [Symbol.nonterminal.injEq, reduceCtorEq]
-      rw [hh]
-    unfold EDT0LGrammar.generates
-    unfold EDT0LGrammar.generates at ih₂
-    unfold EDT0LGrammar.derives
-    unfold EDT0LGrammar.derives at ih₂
-    exact Relation.ReflTransGen.tail ih₂ hh
+  | .lhs _ | .init_lhs | .init_rhs =>
+    unfold Union rewriteSymbol
+    simp only
+    match s with | .terminal _ | .nonterminal _ => simp only
 
-theorem defines_union : data.grammar.language = data.E₀.language + data.E₁.language := by
-  rw [Language.add_def]
-  unfold EDT0LGrammar.language
-  --
-  have h (w : List α) :
-      data.grammar.generates (List.map Symbol.terminal w)
-      ↔ data.E₀.generates (List.map Symbol.terminal w)
-        ∨ data.E₁.generates (List.map Symbol.terminal w) := by
-    --
-    constructor
-    · intro h
-      replace h := data.basic_property _ h
-      match h with
-      | .inl h =>
-        exfalso
-        -- aesop?
-        simp_all only [
-          true_or, List.map_eq_singleton_iff, reduceCtorEq, and_false, exists_false]
-      | .inr (.inl h') =>
-        --
-        replace h := h'
-        clear h'
-        left
-        replace ⟨u, ⟨h_l, h_r⟩⟩ := h
-        have hh : List.map Symbol.terminal w = u := by
-          clear h_r
-          clear h
-          induction u generalizing w
-          · simp_all only [List.map_nil, List.map_eq_nil_iff]
-          · rename_i a as ih
-            -- unfold extend_alphabet₀ at ih
-            simp_all only [List.map_cons]
-            have hh : w ≠ [] := by
-              simp_all only [ne_eq]
-              intro a_1
-              subst a_1
-              simp_all only [List.map_nil, List.nil_eq, reduceCtorEq]
-            replace hh : ∃ b bs, w = b :: bs := by
-              exact List.ne_nil_iff_exists_cons.mp hh
-            replace ⟨b, bs, hh⟩ := hh
-            subst hh
-            unfold List.map
-            conv at h_l =>
-              lhs
-              unfold List.map
-            replace ih := ih bs
-            have h₁ : Symbol.terminal b = @extend_alphabet₀ α V₀ V₁ a := by
-              simp_all only [List.cons.injEq, forall_const]
-            have h₂ :
-                List.map Symbol.terminal bs =
-                List.map (@extend_alphabet₀ α V₀ V₁) as := by
-              simp_all only [List.cons.injEq, true_and, forall_const]
-            replace ih := ih h₂
-            rw [← ih]
-            unfold extend_alphabet₀ at h₁
-            replace h₁ : Symbol.terminal b = a := by
-              match a with
-              | .terminal t =>
-                subst ih
-                simp_all only [
-                  Symbol.terminal.injEq,
-                  List.map_map, List.map_inj_left, Function.comp_apply,
-                  List.cons.injEq, implies_true, and_true]
-              | .nonterminal n =>
-                simp only at h₁
-                exfalso
-                simp_all only [reduceCtorEq]
-            rw [h₁]
-        rw [hh]
-        exact h_r
-      | .inr (.inr h') =>
-        --
-        replace h := h'
-        clear h'
-        right
-        replace ⟨u, ⟨h_l, h_r⟩⟩ := h
-        have hh : List.map Symbol.terminal w = u := by
-          clear h_r
-          clear h
-          induction u generalizing w
-          · simp_all only [List.map_nil, List.map_eq_nil_iff]
-          · rename_i a as ih
-            -- unfold extend_alphabet₀ at ih
-            simp_all only [List.map_cons]
-            have hh : w ≠ [] := by
-              simp_all only [ne_eq]
-              intro a_1
-              subst a_1
-              simp_all only [List.map_nil, List.nil_eq, reduceCtorEq]
-            replace hh : ∃ b bs, w = b :: bs := by
-              exact List.ne_nil_iff_exists_cons.mp hh
-            replace ⟨b, bs, hh⟩ := hh
-            subst hh
-            unfold List.map
-            conv at h_l =>
-              lhs
-              unfold List.map
-            replace ih := ih bs
-            have h₁ : Symbol.terminal b = @extend_alphabet₁ α V₀ V₁ a := by
-              simp_all only [List.cons.injEq, forall_const]
-            have h₂ :
-                List.map Symbol.terminal bs =
-                List.map (@extend_alphabet₁ α V₀ V₁) as := by
-              simp_all only [List.cons.injEq, true_and, forall_const]
-            replace ih := ih h₂
-            rw [← ih]
-            unfold extend_alphabet₁ at h₁
-            replace h₁ : Symbol.terminal b = a := by
-              match a with
-              | .terminal t =>
-                subst ih
-                simp_all only [
-                  Symbol.terminal.injEq,
-                  List.map_map, List.map_inj_left, Function.comp_apply,
-                  List.cons.injEq, implies_true, and_true]
-              | .nonterminal n =>
-                simp only at h₁
-                exfalso
-                simp_all only [reduceCtorEq]
-            rw [h₁]
-        rw [hh]
-        exact h_r
-    · intro h
-      cases h
-      · rename_i h
-        have hh := data.basic_property₀ _ h
-        rw [extend_alphabet₀_terminal_word] at hh
-        exact hh
-      · rename_i h
-        have hh := data.basic_property₁ _ h
-        rw [extend_alphabet₁_terminal_word] at hh
-        exact hh
-  exact Language.ext_iff.mpr h
+variable {α V₀ T₀ V₁ T₁ : Type*} (E₀ : EDT0LGrammar α V₀ T₀) (E₁ : EDT0LGrammar α V₁ T₁) in
+@[simp]
+lemma Union.rewritWord_lhs (t w) :
+    (Union E₀ E₁).rewriteWord t (List.map Union.map_symbol_lhs w) =
+      match t with
+      | .lhs t' =>
+        List.map Union.map_symbol_lhs (E₀.rewriteWord t' w)
+      | .rhs _ | .init_lhs | .init_rhs =>
+        List.map Union.map_symbol_lhs w
+    := by
+  match t with
+  | .lhs t' =>
+    simp only
+    induction w with
+    | nil =>
+      rfl
+    | cons x xs ih =>
+      simp only [List.map_cons, rewriteWord_cons, rewriteSymbol_lhs, List.map_append, ih]
+  | .rhs _ | .init_lhs | .init_rhs =>
+    simp only
+    induction w with
+    | nil =>
+      rfl
+    | cons x xs ih =>
+      simp only [List.map_cons, rewriteWord_cons, rewriteSymbol_lhs, List.cons_append,
+        List.nil_append, ih]
 
-end UnionData
+variable {α V₀ T₀ V₁ T₁ : Type*} (E₀ : EDT0LGrammar α V₀ T₀) (E₁ : EDT0LGrammar α V₁ T₁) in
+@[simp]
+lemma Union.rewritWord_rhs (t w) :
+    (Union E₀ E₁).rewriteWord t (List.map Union.map_symbol_rhs w) =
+      match t with
+      | .rhs t' =>
+        List.map Union.map_symbol_rhs (E₁.rewriteWord t' w)
+      | .lhs _ | .init_lhs | .init_rhs =>
+        List.map Union.map_symbol_rhs w
+    := by
+  match t with
+  | .rhs t' =>
+    simp only
+    induction w with
+    | nil =>
+      rfl
+    | cons x xs ih =>
+      simp only [List.map_cons, rewriteWord_cons, rewriteSymbol_rhs, List.map_append, ih]
+  | .lhs _ | .init_lhs | .init_rhs =>
+    simp only
+    induction w with
+    | nil =>
+      rfl
+    | cons x xs ih =>
+      simp only [List.map_cons, rewriteWord_cons, rewriteSymbol_rhs, List.cons_append,
+        List.nil_append, ih]
 
-theorem closed_under_union (L₁ L₂ : Language α)
+variable {α V₀ T₀ V₁ T₁ : Type*} (E₀ : EDT0LGrammar α V₀ T₀) (E₁ : EDT0LGrammar α V₁ T₁) in
+inductive Union.generatesP (w : List (Symbol α (Union.extended_nonterminals V₀ V₁))) : Prop where
+  | init (h : w = [.nonterminal .init])
+  | lhs (s) (h₁ : w = List.map Union.map_symbol_lhs s) (h₂ : E₀.Generates s)
+  | rhs (s) (h₁ : w = List.map Union.map_symbol_rhs s) (h₂ : E₁.Generates s)
+
+variable {α V₀ T₀ V₁ T₁ : Type*} (E₀ : EDT0LGrammar α V₀ T₀) (E₁ : EDT0LGrammar α V₁ T₁) in
+lemma Union.generates_iff (w) : (Union E₀ E₁).Generates w ↔ Union.generatesP E₀ E₁ w := by
+  constructor
+  · intro h
+    induction h with
+    | refl =>
+      exact .init rfl
+    | tail x y ih =>
+      rename_i u v
+      obtain ⟨t, rfl⟩ := y
+      cases ih with
+      | init ih =>
+        subst ih
+        cases t with
+        | init_lhs =>
+          exact generatesP.lhs E₀.initialWord rfl (generates_initial E₀)
+        | init_rhs =>
+          exact generatesP.rhs E₁.initialWord rfl (generates_initial E₁)
+        | lhs t | rhs t =>
+          exact .init rfl
+      | lhs s h₁ h₂ =>
+        subst h₁
+        refine generatesP.lhs
+          (match t with | .lhs t => E₀.rewriteWord t s | _ => s)
+          ?_ ?_
+        · simp only [rewritWord_lhs]
+          cases t <;> rfl
+        · split
+          · rename_i ht t
+            exact generates_rewriteWord_tail h₂ t
+          · exact h₂
+      | rhs s h₁ h₂ =>
+        subst h₁
+        refine generatesP.rhs
+          (match t with | .rhs t => E₁.rewriteWord t s | _ => s)
+          ?_ ?_
+        · simp only [rewritWord_rhs]
+          cases t <;> rfl
+        · split
+          · rename_i ht t
+            exact generates_rewriteWord_tail h₂ t
+          · exact h₂
+  · intro h
+    cases h with
+    | init h =>
+      subst h
+      exact (Union E₀ E₁).generates_initial
+    | lhs s h₁ h₂ =>
+      subst h₁
+      induction h₂ with
+      | refl =>
+        exact derives_single ⟨.init_lhs, rfl⟩
+      | tail x y ih =>
+        refine derives_tail ih ?_
+        obtain ⟨t, rfl⟩ := y
+        use .lhs t
+        simp only [rewritWord_lhs]
+    | rhs s h₁ h₂ =>
+      subst h₁
+      induction h₂ with
+      | refl =>
+        exact derives_single ⟨.init_rhs, rfl⟩
+      | tail x y ih =>
+        refine derives_tail ih ?_
+        obtain ⟨t, rfl⟩ := y
+        use .rhs t
+        simp only [rewritWord_rhs]
+
+variable {α V₀ T₀ V₁ T₁ : Type*} (E₀ : EDT0LGrammar α V₀ T₀) (E₁ : EDT0LGrammar α V₁ T₁) in
+theorem Union.defines_union : (Union E₀ E₁).language = E₀.language + E₁.language := by
+  ext1 w
+  rw [language_mem_iff, Language.mem_add]
+  constructor
+  · intro h
+    rw [generates_iff] at h
+    cases h with
+    | init h =>
+      simp only [List.map_eq_singleton_iff, reduceCtorEq, and_false, exists_false] at h
+    | lhs s h₁ h₂ =>
+      left
+      obtain rfl : s = List.map .terminal w := by
+        clear h₂
+        induction w generalizing s with
+        | nil =>
+          simp only [List.map_nil, List.nil_eq, List.map_eq_nil_iff] at h₁
+          subst h₁
+          rfl
+        | cons x y ih =>
+          simp only [List.map_cons] at h₁
+          replace h₁ := Eq.symm h₁
+          rw [List.map_eq_cons_iff] at h₁
+          obtain ⟨a, as, rfl, h3,h4⟩ := h₁
+          simp only [List.map_cons, List.cons.injEq]
+          split_ands
+          · unfold map_symbol_lhs at h3
+            split at h3
+            · simp only [Symbol.terminal.injEq] at h3
+              subst h3
+              rfl
+            · simp only [reduceCtorEq] at h3
+          · exact ih as (Eq.symm h4)
+      exact (language_mem_iff E₀).mpr h₂
+    | rhs s h₁ h₂ =>
+      right
+      obtain rfl : s = List.map .terminal w := by
+        clear h₂
+        induction w generalizing s with
+        | nil =>
+          simp only [List.map_nil, List.nil_eq, List.map_eq_nil_iff] at h₁
+          subst h₁
+          rfl
+        | cons x y ih =>
+          simp only [List.map_cons] at h₁
+          replace h₁ := Eq.symm h₁
+          rw [List.map_eq_cons_iff] at h₁
+          obtain ⟨a, as, rfl, h3,h4⟩ := h₁
+          simp only [List.map_cons, List.cons.injEq]
+          split_ands
+          · unfold map_symbol_rhs at h3
+            split at h3
+            · simp only [Symbol.terminal.injEq] at h3
+              subst h3
+              rfl
+            · simp only [reduceCtorEq] at h3
+          · exact ih as (Eq.symm h4)
+      exact (language_mem_iff E₁).mpr h₂
+  · intro h
+    rw [generates_iff]
+    obtain h | h := h
+    · exact .lhs
+        (List.map .terminal w)
+        (by simp only [List.map_map, List.map_inj_left, Function.comp_apply, implies_true])
+        ((language_mem_iff E₀).mp h)
+    · exact .rhs
+        (List.map .terminal w)
+        (by simp only [List.map_map, List.map_inj_left, Function.comp_apply, implies_true])
+        ((language_mem_iff E₁).mp h)
+
+end EDT0LGrammar
+
+theorem Language.isEDT0L_union {α} (L₁ L₂ : Language α)
   (h₁ : L₁.IsEDT0L)
   (h₂ : L₂.IsEDT0L) :
     (L₁ + L₂).IsEDT0L := by
   have ⟨_, _ , E₁, P₁⟩ := h₁
   have ⟨_, _ , E₂, P₂⟩ := h₂
-  let union_data := UnionData.mk E₁ E₂
-  have h := union_data.defines_union
-  have ⟨n,m,E',P'⟩ := union_data.grammar.edt0l_grammars_generate_edt0l_languages
+  have h := EDT0LGrammar.Union.defines_union E₁ E₂
+  have ⟨n, m, E', P'⟩ := (EDT0LGrammar.Union E₁ E₂).language_isEDT0L
   use n, m, E'
-  rw [P', h]
-  unfold union_data
-  rw [P₁, P₂]
+  rw [P', h, P₁, P₂]
 
-end EDT0LGrammar
