LSystems/FiniteIndexEDT0L/LULT/Defs.lean
@@ -3,164 +3,110 @@ Copyright (c) 2025 Alex Bishop. All rights reserved.
 Released under Apache 2.0 license as described in the file LICENSE.
 Author: Alex Bishop
 -/
-import LSystems.EDT0L.Defs
-import LSystems.EDT0L.DeriveSequence
+module
+
+public import LSystems.EDT0L.Defs
+public import LSystems.EDT0L.Basic
+public import LSystems.EDT0L.RewriteSequence
+
+@[expose] public section
 
 namespace EDT0LGrammar
 
-def ContainedAtMostOnce {α : Type*} (a : α) (s : List α) : Prop :=
-  a ∉ s ∨ ∃ s₁ s₂ : List α, a ∉ s₁ ∧ a ∉ s₂ ∧ s = s₁ ++ [a] ++ s₂
-
-@[simp]
-lemma containedAtMostOnce_iff_count_le_one {α : Type*} [DecidableEq α] (a : α) (s) :
-    ContainedAtMostOnce a s ↔ s.count a ≤ 1 := by
-  constructor
-  · intro h
-    obtain h | h := h
-    · rw [Nat.le_one_iff_eq_zero_or_eq_one]
-      left
-      exact List.count_eq_zero.mpr h
-    · rw [Nat.le_one_iff_eq_zero_or_eq_one]
-      right
-      obtain ⟨s₁, s₂, h₁, h₂, rfl⟩ := h
-      simp only [List.append_assoc, List.cons_append, List.nil_append, List.count_append,
-        List.count_cons_self]
-      replace h₁ := List.count_eq_zero.mpr h₁
-      replace h₂ := List.count_eq_zero.mpr h₂
-      rw [h₁, h₂]
-  · intro h
-    rw [Nat.le_one_iff_eq_zero_or_eq_one] at h
-    obtain h | h := h
-    · unfold ContainedAtMostOnce
-      left
-      exact List.count_eq_zero.mp h
-    · unfold ContainedAtMostOnce
-      right
-      let idx? := s.finIdxOf? a
-      cases h₁ : idx? with
-      | none =>
-        exfalso
-        unfold idx? at h₁
-        replace h : a ∈ s := by
-          clear * - h
-          by_contra contra
-          replace contra := List.count_eq_zero.mpr contra
-          rw [h] at contra
-          simp only [one_ne_zero] at contra
-        exact List.finIdxOf?_eq_none_iff.mp h₁ h
-      | some i =>
-        unfold idx? at h₁
-        replace ⟨h₁, _⟩ := List.finIdxOf?_eq_some_iff.mp h₁
-        have h₂ : s = s.take i ++ [s[i]] ++ s.drop (i + 1) := by
-          simp only [Fin.getElem_fin, List.take_append_getElem, List.take_append_drop]
-        --
-        rw [h₁] at h₂
-        rw [h₂] at h
-        simp only [List.append_assoc, List.cons_append, List.nil_append, List.count_append,
-          List.count_cons_self] at h
-        simp only [← Nat.add_assoc, Nat.add_eq_right, Nat.add_eq_zero] at h
-        --
-        have ⟨h_l, h_r⟩ := h
-        --
-        use
-          s.take i,
-          s.drop (i + 1),
-          List.count_eq_zero.mp h_l,
-          List.count_eq_zero.mp h_r,
-          h₂
-
-def IsLULT {α V T : Type*} [Fintype V] [Fintype T] (E : EDT0LGrammar α V T) : Prop :=
+def IsLULT {α V T : Type*} [BEq V] (E : EDT0LGrammar α V T) : Prop :=
   ∀ w ∈ E.language,
-  ∃ (a : List T) (_ : E.deriveSeq a [.nonterminal E.initial] = w.map .terminal),
-    ∀ (i : ℕ) (_ : i ≤ a.length),
-      let a₁ := a.take i;
-      let a₂ := a.drop i;
-      ∀ v : V,
-        let before_split := E.deriveSeq a₁ [.nonterminal E.initial];
-        let after_split := E.deriveSeq a₂ [.nonterminal v];
-        (ContainedAtMostOnce (.nonterminal v) before_split) ∨ (after_split.length ≤ 1)
+    ∃ (s : List T),
+      E.rewriteSeq s E.initialWord = w.map .terminal ∧
+      ∀ (v : V) (i : ℕ),
+        i ≤ s.length →
+          (filterNonterminals (E.rewriteSeq (s.take i) E.initialWord)).count v ≤ 1 ∨
+          (E.rewriteSeq (s.drop i) [.nonterminal v]).length ≤ 1
 
 end EDT0LGrammar
 
 def Language.IsLULT {α : Type*} (L : Language α) : Prop :=
-  ∃ n m : ℕ, ∃ E : EDT0LGrammar α (Fin n) (Fin m), ∃ _ : E.IsLULT, E.language = L
+  ∃ n m : ℕ, ∃ E : EDT0LGrammar α (Fin n) (Fin m), E.IsLULT ∧ E.language = L
 
 namespace EDT0LGrammar
-namespace EquivData
-variable {α V T V' T' : Type*}
-  [Fintype V] [Fintype T] [Fintype V'] [Fintype T']
-  [DecidableEq α] [DecidableEq V] [DecidableEq V']
-variable (data : @EquivData α V T V' T' _ _ _ _)
+variable {α V T : Type*} [BEq V] [LawfulBEq V] (E : EDT0LGrammar α V T)
 
-lemma equiv_preserves_lult (h : data.E.IsLULT) : data.grammar.IsLULT := by
-  unfold IsLULT
-  intro w w_in_lang
-  replace ⟨a, a', h⟩ := h w (by rw [equiv_eq_language]; exact w_in_lang)
-  use data.equivTableSeq a
-  use (by
-    rw [deriveSeq_equiv']
-    simp only [Equiv.symm_apply_apply, equivWord_symm_cons, equiv_symbol_nonterminal',
-      equivV_grammar_initial, equivWord_symm_nil]
-    rw [a']
-    simp only [equivWord_terminals])
+private lemma equiv_isLULT {α' V' T'} [BEq V'] [LawfulBEq V']
+  (equivα : α ≃ α') (equivV : V ≃ V') (equivT : T ≃ T')
+  (h : E.IsLULT) :
+    (E.equiv equivα equivV equivT).IsLULT := by
+  classical
+  intro w hw
+  have ⟨s, h', h''⟩ := h (w.map equivα.symm) (by
+    rw [equiv_language] at hw
+    obtain ⟨w', hw, rfl⟩ := hw
+    simpa )
   --
-  simp only
-  intro i hi v
-  simp only [equivTableSeq_length] at hi
-  --
-  replace h := h i hi (data.equivV.symm v)
-  simp only at h
-  --
-  obtain h | h := h
-  · left
-    simp only [containedAtMostOnce_iff_count_le_one] at h
-    simp only [containedAtMostOnce_iff_count_le_one]
-    change
-      let x := _
-      let s := _
-      List.count x s ≤ 1
-    extract_lets x s
-    --
-    have h₁ := List.count_map_of_injective
-      s
-      (data.equivSymbol.invFun)
-      (by
-        simp only [Equiv.invFun_as_coe]
-        exact Equiv.injective data.equivSymbol.symm)
-      x
-    rw [← h₁]
-    subst x s
-    simp only [Equiv.invFun_as_coe, equiv_symbol_nonterminal']
-    clear * - h
-    --
-    change List.count _ (data.equivWord.symm _) ≤ 1
-    rw [deriveSeq_equiv] at h
-    simp only [equivWord_cons, equiv_symbol_nonterminal, equivV_initial, equivWord_nil] at h
-    --
-    conv at h =>
+  use s.map equivT
+  constructor
+  · simp only [equiv_initialWord, equivWord_cons, equivSymbol_nonterminal, equivWord_nil,
+      equiv_rewriteSeq', List.map_map, Equiv.symm_comp_self, List.map_id_fun, id_eq,
+      ← equivWord_symm]
+    conv =>
       lhs
       arg 2
-      arg 2
-      arg 2
-      change List.map _ _
-      rw [List.map_take]
-      change List.take _ (data.equivTableSeq a)
-    exact h
-  · right
-    rw [deriveSeq_equiv] at h
-    simp only [equivWord_cons, equiv_symbol_nonterminal, Equiv.apply_symm_apply, equivWord_nil] at h
-    conv at h =>
-      lhs
-      arg 1
-      arg 2
-      arg 2
-      change List.map _ _
-      rw [List.map_drop]
-      change List.drop _ (data.equivTableSeq _)
-    change (List.map _ _).length ≤ 1 at h
-    rw [List.length_map] at h
-    exact h
+      unfold equivWord
+      simp only [Equiv.symm_mk, Equiv.coe_fn_mk, List.map_cons, equivSymbol_nonterminal,
+        Equiv.symm_apply_apply, List.map_nil]
+      arg 3
+      change E.initialWord
+    rw [h']
+    unfold equivWord
+    simp
+  · intro v' i' hi'
+    replace h'' := h'' (equivV.symm v') i' (by simp_all)
+    obtain h'' | h'' := h''
+    · left
+      clear * - h''
+      simp only [equiv_initialWord, equivWord_cons, equivSymbol_nonterminal, equivWord_nil,
+        equiv_rewriteSeq', List.map_take, List.map_map, Equiv.symm_comp_self, List.map_id_fun,
+        id_eq, ← equivWord_symm, filterNonterminals_equivWord]
+      unfold equivWord
+      conv =>
+        lhs ; arg 2; arg 2; arg 1; arg 3
+        simp only [Equiv.symm_mk, Equiv.coe_fn_mk, List.map_cons, equivSymbol_nonterminal,
+          Equiv.symm_apply_apply, List.map_nil]
+        change E.initialWord
+      rw [List.count, List.countP_map]
+      change let f : _ → _ := _ ; List.countP f _ ≤ _
+      intro f
+      have : f = fun x ↦ x == equivV.symm v' := by
+        funext x
+        subst f
+        clear * -
+        simp only [Function.comp_apply, beq_eq_beq]
+        exact Equiv.apply_eq_iff_eq_symm_apply equivV
+      rw [this]
+      change List.count _ _ ≤ _
+      exact h''
+    · right
+      clear * - h''
+      simpa
 
-end EquivData
+lemma equiv_isLULT_iff {α' V' T'} [BEq V'] [LawfulBEq V']
+  (equivα : α ≃ α') (equivV : V ≃ V') (equivT : T ≃ T') :
+    E.IsLULT ↔ (E.equiv equivα equivV equivT).IsLULT := by
+  classical
+  constructor
+  · exact equiv_isLULT E equivα equivV equivT
+  · let E' := (equiv equivα equivV equivT) E
+    have h' : E = (equiv equivα.symm equivV.symm equivT.symm) E' :=
+      (Equiv.symm_apply_eq (equiv equivα.symm equivV.symm equivT.symm)).mp rfl
+    conv => intro x ; rw [h']
+    change E'.IsLULT → _
+    exact equiv_isLULT E' equivα.symm equivV.symm equivT.symm
+
+theorem lult_language_isLULT [Finite V] [Finite T] :
+    E.IsLULT → E.language.IsLULT := by
+  intro h
+  have := Fintype.ofFinite V
+  have := Fintype.ofFinite T
+  have h' := equiv_language_eq_language (Fintype.equivFin V) (Fintype.equivFin T) E
+  unfold Language.IsLULT
+  exact ⟨_, _ , _,  equiv_isLULT E (Equiv.refl α) _ _ h, h'⟩
 
 end EDT0LGrammar
