LSystems/StringTransducer/Defs.lean
@@ -3,77 +3,233 @@ Copyright (c) 2025 Alex Bishop. All rights reserved.
 Released under Apache 2.0 license as described in the file LICENSE.
 Author: Alex Bishop
 -/
-import Mathlib.Computability.Language
+module
 
-structure StringTransducer (α β σ : Type*) [Fintype α] [Fintype β] [Fintype σ] where
+public import Mathlib.Computability.Language
+
+@[expose] public section
+
+structure StringTransducer (α β σ : Type*) where
   start : σ
-  accept : Finset σ
+  accept : Set σ
   step : σ → α → (σ × List β)
-  final : (q : σ) → q ∈ accept → List β
+  final : (q : σ) → (h : q ∈ accept) → List β
 
 namespace StringTransducer
-variable {α β σ : Type*} [Fintype α] [Fintype β] [Fintype σ]
-variable (𝓣 : StringTransducer α β σ)
+variable {α β σ} (S : StringTransducer α β σ)
 
-def RewriteWordWithoutFinal : σ → List α → σ × List β
+@[simp]
+def rewriteWithoutFinal : σ → List α → σ × List β
   | q, [] => (q, [])
   | q, a :: as =>
-    let ⟨q_next, head⟩ := 𝓣.step q a;
-    let ⟨q_last, tail⟩ := RewriteWordWithoutFinal q_next as;
+    let ⟨q_next, head⟩ := S.step q a;
+    let ⟨q_last, tail⟩ := rewriteWithoutFinal q_next as;
     (q_last, head ++ tail)
 
-def Generates (source : List α) (target : List β) : Prop :=
-  let ⟨q, w⟩ := 𝓣.RewriteWordWithoutFinal 𝓣.start source
-  ∃ h : q ∈ 𝓣.accept, target = w ++ 𝓣.final q h
-
-def map (L : Language α) : Language β := 
-  { w : List β | ∃ u ∈ L, 𝓣.Generates u w}
-
-namespace RewriteWordWithoutFinal
-
 @[simp]
-lemma refl (q : σ) : 𝓣.RewriteWordWithoutFinal q [] = (q, []) := rfl
+lemma rewriteWithoutFinal_append (q : σ) (u v : List α) :
+    S.rewriteWithoutFinal q (u ++ v) =
+      let ⟨q',u'⟩ := S.rewriteWithoutFinal q u
+      let ⟨q'',v'⟩ := S.rewriteWithoutFinal q' v
+      (q'', u' ++ v') := by
+  split
+  rename_i x q_last tail hq
+  split
+  rename_i x' q_last' tail' hq'
+  induction u generalizing q tail with
+  | nil =>
+    simp only [List.nil_append]
+    simp only [rewriteWithoutFinal, Prod.mk.injEq, List.nil_eq] at hq
+    obtain ⟨rfl, rfl⟩ := hq
+    simpa using hq'
+  | cons x xs ih =>
+    simp only [List.cons_append, rewriteWithoutFinal, Prod.mk.injEq]
+    simp only [rewriteWithoutFinal, Prod.mk.injEq] at hq
+    replace ih := ih (S.3 q x).1 (S.rewriteWithoutFinal (S.3 q x).1 xs).2 (by
+      obtain ⟨rfl, _ ⟩ := hq
+      rfl)
+    grind only
 
-lemma single (q : σ) (a : α) :
-    𝓣.RewriteWordWithoutFinal q [a] = 𝓣.step q a := by
-  unfold RewriteWordWithoutFinal
-  simp only [refl, List.append_nil]
+def rewrite [DecidablePred (· ∈ S.accept)] (source : List α) : Option (List β) :=
+  let ⟨q,w⟩ := S.rewriteWithoutFinal S.start source
+  if h : q ∈ S.accept then w ++ S.final q h else .none
 
-@[simp]
-lemma cons (q : σ) (a : α) (as : List α) :
-    let status₁ := 𝓣.RewriteWordWithoutFinal q [a];
-    let status₂ := 𝓣.RewriteWordWithoutFinal status₁.1 as;
+def Rewrites (source : List α) (target : List β) : Prop :=
+  let ⟨q,w⟩ := S.rewriteWithoutFinal S.start source
+  ∃ h : q ∈ S.accept, target = w ++ S.final q h
+
+lemma rewrite_eq_Rewrites [DecidablePred (· ∈ S.accept)] (source : List α) (target : List β) :
+    S.Rewrites source target ↔ S.rewrite source = target := by
+  simp only [Rewrites, rewrite, Option.dite_none_right_eq_some, Option.some.injEq]
+  tauto
+
+def map (L : Language α) : Language β := { w : List β | ∃ u ∈ L, S.Rewrites u w}
+
+end StringTransducer
+
+def Function.IsStringTransduction {α β} (f : Language α → Language β) : Prop :=
+  ∃ (n : ℕ), ∃ (S : StringTransducer α β (Fin n)), ∀ (L : Language α), f L = S.map L
+
+namespace StringTransducer
+
+variable {α β σ} [Finite σ] (S : StringTransducer α β σ) in
+lemma map_isStringTransduction : Function.IsStringTransduction S.map := by
+
+  sorry
+
+
+structure Compose.accept_prop {α β₁ β₂ σ₁ σ₂}
+    (S₁ : StringTransducer α β₁ σ₁) (S₂ : StringTransducer β₁ β₂ σ₂)
+    (q₁ : σ₁) (q₂ : σ₂) : Prop where
+  q₁_accepts : q₁ ∈ S₁.accept
+  q₂_leads_to_accept: (S₂.rewriteWithoutFinal q₂ (S₁.final q₁ q₁_accepts)).1 ∈ S₂.accept
+
+def Compose {α β₁ β₂ σ₁ σ₂} (S₁ : StringTransducer α β₁ σ₁) (S₂ : StringTransducer β₁ β₂ σ₂) :
+    StringTransducer α β₂ (σ₁ × σ₂) where
+  start := ⟨S₁.start, S₂.start⟩
+  accept :=  { ⟨q₁,q₂⟩ : σ₁ × σ₂ | Compose.accept_prop S₁ S₂ q₁ q₂ }
+  step := fun (q : σ₁ × σ₂) (a : α) ↦
+    let ⟨q_in₁, q_in₂⟩ := q
+    let ⟨q_out₁, w_out₁⟩ := S₁.step q_in₁ a
+    let ⟨q_out₂, w_out₂⟩ := S₂.rewriteWithoutFinal q_in₂ w_out₁
+    ⟨⟨q_out₁, q_out₂⟩, w_out₂⟩
+  final := fun (q : σ₁ × σ₂) h ↦
+    let ⟨q₁, q₂⟩ := q
+    have h' : Compose.accept_prop S₁ S₂ q₁ q₂ := h
     --
-    𝓣.RewriteWordWithoutFinal q (a::as) = ⟨status₂.1, status₁.2 ++ status₂.2⟩ := by
-  intro status₁ status₂
-  unfold RewriteWordWithoutFinal
-  split
-  rename_i q' a' h₁
-  split
-  rename_i q'' as' h₂
-  --
-  subst status₁
-  subst status₂
-  --
-  ext1 <;> (simp only; rw [single, h₁, h₂])
+    let final₁ := S₁.final q₁ h'.q₁_accepts
+    --
+    let tmp₂ := S₂.rewriteWithoutFinal q₂ final₁
+    let q₂' := tmp₂.1
+    let pre_final₂ := tmp₂.2
+    --
+    let final₂ := S₂.final q₂' (h'.q₂_leads_to_accept)
+    --
+    pre_final₂ ++ final₂
 
--- lemma append (q : σ) (a b : List α) :
---     let status₁ := 𝓣.RewriteWordWithoutFinal q a;
---     let status₂ := 𝓣.RewriteWordWithoutFinal status₁.1 b;
+-- lemma Compose.left {α β₁ β₂ σ₁ σ₂}
+--   (S₁ : StringTransducer α β₁ σ₁) [DecidablePred (· ∈ S₁.accept)]
+--   (S₂ : StringTransducer β₁ β₂ σ₂) {u v} :
+--     (S₁.Compose S₂).Rewrites u v → S₁.rewrite u ≠ .none := by
+--   classical
+--   -- intro h contra
+--   -- unfold rewrite at contra
+--   -- extract_lets wq q w at contra
+--   -- split at contra
+--   -- · trivial
+--   -- --
+--   -- rename_i hq
+--   -- subst wq w q
+--   -- --
+--   -- rw [rewrite_eq_Rewrites, rewrite] at h
+--   -- split at h
+--   -- rotate_right
+--   -- · trivial
+--   -- --
+--   -- rename_i hq'
+--   -- clear * - hq hq'
+--   -- have : ((S₁.Compose S₂).rewriteWithoutFinal (S₁.Compose S₂).start u).1.1
+--   --           = (S₁.rewriteWithoutFinal S₁.start u).1 := by
+--   --   induction u using List.reverseRec with
+--   --   | nil =>
+--   --     rfl
+--   --   | append_singleton xs x ih =>
+--   --     simp only [rewriteWithoutFinal_append, rewriteWithoutFinal, List.append_nil, Prod.mk.eta]
+--   --     simp only [rewriteWithoutFinal_append, rewriteWithoutFinal, List.append_nil,
+--   --       Prod.mk.eta] at hq'
+--   --     
+--   --
+--   --     sorry
+--
+--   sorry
+
+lemma Compose.defined {α β₁ β₂ σ₁ σ₂}
+  (S₁ : StringTransducer α β₁ σ₁) (S₂ : StringTransducer β₁ β₂ σ₂) :
+    (Compose S₁ S₂).map = S₂.map ∘ S₁.map := by
+  classical
+  funext L
+  ext1 w
+  constructor
+  · intro h
+    unfold map at ⊢ h
+    unfold Compose at h
+    simp_all only [Set.mem_setOf_eq, Function.comp_apply]
+    --
+    change let f : _ → _ := _ ; w ∈ {w | f w} at h
+    extract_lets f at h
+    change f w at h
+    subst f
+    obtain ⟨u, hu, h⟩ := h
+    --
+    change let f : _ → _ := _ ; w ∈ {w | f w}
+    extract_lets f
+    change f w
+    subst f
+    simp only
+    conv =>
+      arg 1
+      intro u
+      lhs
+      tactic =>
+        change let f : _ → _ := _ ; (u ∈ {w | f w}) = _
+        extract_lets f
+        change f u = _
+        subst f
+    simp only [rewrite_eq_Rewrites]
+    simp only [rewrite_eq_Rewrites] at h
+    
+
+    sorry
+  · intro h
+
+    sorry
+
+
+
+
+end StringTransducer 
+
+
+-- @[simp]
+-- lemma rewriteWithoutFinal_nil (q : σ) : S.rewriteWithoutFinal q [] = (q, []) := rfl
+--
+-- @[simp]
+-- lemma rewriteWithoutFinal_single (q : σ) (a : α) :
+--     st.rewriteWithoutFinal q [a] = st.step q a := by
+--   unfold rewriteWithoutFinal
+--   simp only [rewriteWithoutFinal_nil, List.append_nil]
+--
+-- lemma rewriteWithoutFinal_cons (q : σ) (a : α) (as : List α) :
+--     let status₁ := st.rewriteWithoutFinal q [a];
+--     let status₂ := st.rewriteWithoutFinal status₁.1 as;
 --     --
---     𝓣.RewriteWordWithoutFinal q (a ++ b) = ⟨status₂.1, status₁.2 ++ status₂.2⟩ := by
+--     st.rewriteWithoutFinal q (a::as) = ⟨status₂.1, status₁.2 ++ status₂.2⟩ := by
 --   intro status₁ status₂
+--   unfold rewriteWithoutFinal
+--   split
+--   rename_i q' a' h₁
+--   split
+--   rename_i q'' as' h₂
+--   --
+--   subst status₁
+--   subst status₂
+--   --
+--   ext1 <;> (simp only; rw [rewriteWithoutFinal_single, h₁, h₂])
+
+-- lemma rewriteWithoutFinal_append (q : σ) (a b : List α) :
+--     let status₁ := st.rewriteWithoutFinal q a;
+--     let status₂ := st.rewriteWithoutFinal status₁.1 b;
+--     --
+--     st.rewriteWithoutFinal q (a ++ b) = ⟨status₂.1, status₁.2 ++ status₂.2⟩ := by
 --   induction a with
 --   | nil =>
---     subst status₁ status₂
---     simp only [refl, List.nil_append]
+--     simp only [List.nil_append, rewriteWithoutFinal_nil]
 --   | cons a as ih =>
---     extract_lets status₁' status₂' at ih
---     rw [List.cons_append, cons]
---     -- simp only [ih]
+--     extract_lets s₁ s₂
+--     extract_lets t₁ t₂ at ih
+--     rw [List.cons_append]
+--     conv => lhs; rw [rewriteWithoutFinal_cons]
 --
 --     sorry
 
 
-end RewriteWordWithoutFinal
-end StringTransducer
