LSystems.lean
@@ -5,4 +5,3 @@ Author: Alex Bishop
 -/
 import LSystems.EDT0L
 import LSystems.FiniteIndexEDT0L
-import LSystems.StringTransducer
