LSystems/EDT0L.lean
@@ -1,12 +1,15 @@
 /-
 Copyright (c) 2025 Alex Bishop. All rights reserved.
 Released under Apache 2.0 license as described in the file LICENSE.
-Author: Alex Bishop
+Authors: Alex Bishop
 -/
 import LSystems.EDT0L.Defs
 import LSystems.EDT0L.Basic
 import LSystems.EDT0L.DeadEnds
-import LSystems.EDT0L.DeriveSequence
+import LSystems.EDT0L.RewriteSequence
+import LSystems.EDT0L.Attach
+import LSystems.EDT0L.Mapped
 import LSystems.EDT0L.Union
+import LSystems.EDT0L.RegularLanguage
 
 
