LSystems/EDT0L/Attach.lean
@@ -1,0 +1,180 @@
+/-
+Copyright (c) 2025 Alex Bishop. All rights reserved.
+Released under Apache 2.0 license as described in the file LICENSE.
+Author: Alex Bishop
+-/
+module
+
+public import LSystems.EDT0L.Defs
+public import Mathlib.Data.Finset.Lattice.Fold
+public import LSystems.EDT0L.RewriteSequence
+public import LSystems.EDT0L.Mapped
+
+@[expose] public section
+
+namespace EDT0LGrammar
+
+abbrev visibleα {α V T} (E : EDT0LGrammar α V T) :=
+  { a : α // ∃ (t : T) (v : V), .terminal a ∈  E.table t v}
+
+instance {α V T} [Fintype V] [Fintype T] [DecidableEq α]
+  (E : EDT0LGrammar α V T) : Fintype E.visibleα where
+  elems :=
+    Fintype.elems.sup fun (t : T) ↦
+    Fintype.elems.sup fun (v : V) ↦
+    ((E.table t v).attach.filterMap
+      (fun | ⟨.terminal a, h⟩ => some ⟨a, ⟨_,_,h⟩⟩ | ⟨.nonterminal _, _⟩ => none)).toFinset
+  complete := by
+    intro x
+    simp only [Finset.mem_sup, List.mem_toFinset, List.mem_filterMap, List.mem_attach, true_and,
+      Subtype.exists]
+    have ⟨t,v,h⟩ := x.prop
+    exact ⟨t, Fintype.complete _, v, Fintype.complete _, .terminal ↑x, h, rfl⟩
+
+def attach {α V T} (E : EDT0LGrammar α V T) : EDT0LGrammar E.visibleα V T where
+  initial := E.initial
+  table :=
+    fun t v ↦
+      (E.table t v).attach.map
+        fun | ⟨.terminal a, h⟩ => .terminal ⟨a, ⟨_,_,h⟩⟩ | ⟨.nonterminal v,_⟩ => .nonterminal v
+
+@[simp]
+lemma attach_map {α V T} (E : EDT0LGrammar α V T) : Mapped Subtype.val E.attach = E := by
+  ext1
+  · rfl
+  · funext t v
+    unfold Mapped attach mapWord
+    simp only [List.map_map]
+    change let f : _ → _ := _ ; List.map f _ = _
+    intro f
+    have : f = Subtype.val := by
+      subst f
+      ext1 x
+      simp only [Function.comp_apply]
+      split <;> rename_i heq <;> split at heq <;> grind
+    rw [this]
+    simp
+
+def unattachSymbolWord {α V T} {E : EDT0LGrammar α V T} :
+    List (Symbol E.visibleα V) → List (Symbol α V) :=
+  List.map (fun | .terminal a => .terminal a.val | .nonterminal v => .nonterminal v)
+
+@[simp]
+lemma unattachSymbolWord_initialWord {α V T} {E : EDT0LGrammar α V T} :
+    unattachSymbolWord E.attach.initialWord = E.initialWord := rfl
+
+@[simp]
+lemma unattachSymbolWord_cons {α V T} {E : EDT0LGrammar α V T}
+  {x : Symbol E.visibleα V} {xs : List (Symbol E.visibleα V)} :
+    unattachSymbolWord (x::xs) =
+      (match x with | .terminal a => .terminal a.val | .nonterminal v => .nonterminal v)
+      ::unattachSymbolWord xs := rfl
+
+@[simp]
+lemma unattachSymbolWord_nil {α V T} {E : EDT0LGrammar α V T} :
+    unattachSymbolWord (E := E) [] = [] := rfl
+
+@[simp]
+lemma unattachSymbolWord_append {α V T} {E : EDT0LGrammar α V T}
+  {x y : List (Symbol E.visibleα V)} :
+    unattachSymbolWord (x ++ y) = unattachSymbolWord x ++ unattachSymbolWord y := List.map_append
+
+lemma unattachSymbolWord_congr {α V T} {E : EDT0LGrammar α V T} {u v : List (Symbol E.visibleα V)}
+  (h : unattachSymbolWord u = unattachSymbolWord v) :
+    u = v :=
+  let rec go :
+      (u v : List (Symbol E.visibleα V)) →
+      (h : unattachSymbolWord u = unattachSymbolWord v) →
+      u = v
+    | [],[],_ => rfl
+    | a::as, b::bs, h => by
+      simp only [unattachSymbolWord_cons, List.cons.injEq] at h
+      obtain ⟨h1, h2⟩ := h
+      have R := go as bs h2
+      rw [R]
+      simp only [List.cons.injEq, and_true]
+      split at h1 <;> split at h1
+      · simp_all only [Symbol.terminal.injEq]
+        exact Subtype.ext h1
+      · simp_all
+      · simp_all
+      · simp_all
+    | [], _::_, h => by simp at h
+    |  _::_, [], h => by simp at h
+  go u v h
+
+@[simp]
+lemma unattachSymbolWord_length {α V T} {E : EDT0LGrammar α V T} {w : List (Symbol E.visibleα V)} :
+    (unattachSymbolWord w).length = w.length := by
+  simp [unattachSymbolWord]
+
+@[simp]
+lemma unattachSymbolWord_terminals {α V T} {E : EDT0LGrammar α V T} (w : List E.visibleα) :
+    unattachSymbolWord (w.map .terminal) = w.unattach.map .terminal := by
+  induction w with
+  | nil => rfl
+  | cons a as ih => simp [ih]
+
+@[simp]
+lemma filterNonterminals_unattachSymbolWord {α V T} {E : EDT0LGrammar α V T}
+  (w : List (Symbol E.visibleα V)) :
+    filterNonterminals (unattachSymbolWord w) = filterNonterminals w := by
+  induction w with
+  | nil =>
+    rfl
+  | cons x xs ih =>
+    simp only [unattachSymbolWord_cons, filterNonterminals_cons]
+    split <;> rename_i heq <;> split at heq <;> simp_all
+
+lemma attach_rewriteWord {α V T} (E : EDT0LGrammar α V T) (w : List (Symbol α V))
+  (w' : List (Symbol E.visibleα V)) (h : w = unattachSymbolWord w') (t : T) :
+    E.rewriteWord t w = unattachSymbolWord (E.attach.rewriteWord t w') := by
+  subst h
+  induction w' with
+  | nil =>
+    rfl
+  | cons x xs ih =>
+    simp only [unattachSymbolWord_cons, rewriteWord_cons, ih, unattachSymbolWord_append,
+      List.append_cancel_right_eq]
+    split
+    · rfl
+    · rename_i v
+      unfold attach unattachSymbolWord
+      simp only [rewriteSymbol_nonterminal, List.map_map]
+      change let f : _ → _ := _ ; _ = List.map f _
+      intro f
+      have : f = Subtype.val := by
+        subst f
+        funext x
+        simp only [Function.comp_apply]
+        split
+        · rename_i a heq
+          split at heq
+          · rename_i a' h'
+            simp only [Symbol.terminal.injEq] at ⊢ heq
+            subst heq
+            rfl
+          · rename_i n prop
+            simp at ⊢ heq
+        · rename_i v heq
+          split at heq
+          · simp at heq
+          · simp only [Symbol.nonterminal.injEq] at ⊢ heq
+            exact Eq.symm heq
+      rw [this]
+      simp
+
+lemma attach_rewriteSeq {α V T} (E : EDT0LGrammar α V T) (w : List (Symbol α V))
+  (w' : List (Symbol E.visibleα V)) (h : w = unattachSymbolWord w') (t : List T) :
+    E.rewriteSeq t w = unattachSymbolWord (E.attach.rewriteSeq t w') := by
+  induction t using List.reverseRecOn with
+  | nil =>
+    simpa using h
+  | append_singleton xs x ih =>
+    simp only [rewriteSeq_seq_append, ih, rewriteSeq_seq_cons, rewriteSeq_refl]
+    exact attach_rewriteWord E _ _ rfl x
+
+lemma language_eq_attach_language_map_val {α V T} (E : EDT0LGrammar α V T) :
+    E.attach.language.map Subtype.val = E.language := by simp [← mapped_language]
+
+end EDT0LGrammar
