LSystems/EDT0L/Mapped.lean
@@ -1,0 +1,133 @@
+/-
+Copyright (c) 2025 Alex Bishop. All rights reserved.
+Released under Apache 2.0 license as described in the file LICENSE.
+Author: Alex Bishop
+-/
+module
+
+public import LSystems.EDT0L.Defs
+public import LSystems.EDT0L.Basic
+public import LSystems.EDT0L.RewriteSequence
+
+@[expose] public section
+
+namespace EDT0LGrammar
+
+def mapWord {α α' V} (f : α → α') : List (Symbol α V) → List (Symbol α' V) :=
+  List.map fun | .terminal a => .terminal (f a) | .nonterminal v => .nonterminal v
+
+@[simp]
+lemma mapWord_nil {α α' V} (f : α → α') : mapWord (V := V) f [] = [] := rfl
+
+@[simp]
+lemma mapWord_cons {α α' V} (f : α → α') (x : Symbol α V) (xs : List (Symbol α V)) :
+    mapWord f (x::xs) =
+      (match x with | .terminal a => .terminal (f a) | .nonterminal v => .nonterminal v)
+      :: mapWord f xs := rfl
+
+@[simp]
+lemma mapWord_append {α α' V} (f : α → α') (x y : List (Symbol α V)) :
+    mapWord f (x ++ y) = mapWord f x ++ mapWord f y := List.map_append
+
+lemma mapWord_terminals {α α' V} (f : α → α') (w : List α) :
+    mapWord (V := V) f (w.map .terminal) = w.map (fun x ↦ .terminal (f x)) := by
+  induction w with
+  | nil => rfl
+  | cons x xs ih => simp [ih]
+
+lemma mapWord_eq_terminals {α α' V} (f : α → α') (w : List α') (v : List (Symbol α V))
+  (h : mapWord f v = List.map Symbol.terminal w) :
+    ∃ (u : List α), v = u.map .terminal :=
+  let rec go :
+      (w : List α') →
+      (v : List (Symbol α V)) →
+      (h : mapWord f v = List.map Symbol.terminal w) →
+      ∃ (u : List α), v = u.map .terminal
+    | [], [], h => ⟨[], rfl⟩
+    | a::as, b::bs, h => by
+      simp only [mapWord_cons, List.map_cons, List.cons.injEq] at h
+      obtain ⟨h1, h2⟩ := h
+      obtain ⟨u', hu'⟩ := go as bs h2
+      split at h1
+      · rename_i a'
+        simp only [Symbol.terminal.injEq] at h1
+        use a'::u'
+        simpa using hu'
+      · trivial
+    | _::_, [], h => by simp_all
+    | [], _::_, h => by simp_all
+  go w v h
+
+@[simp]
+lemma filterNonterminals_mapWord {α α' V} (f : α → α') (w : List (Symbol α V)) :
+    filterNonterminals (mapWord f w) = filterNonterminals w := by
+  induction w with
+  | nil =>
+    rfl
+  | cons x xs ih =>
+    simp only [mapWord_cons, filterNonterminals_cons, ih]
+    split <;> rename_i heq <;> split at heq <;> simp_all
+
+def Mapped {α α' V T} (f : α → α') (E : EDT0LGrammar α V T) : EDT0LGrammar α' V T where
+  initial := E.initial
+  table := fun t v ↦ mapWord f (E.table t v)
+
+@[simp]
+lemma mapped_initialWord {α α' V T} (f : α → α') (E : EDT0LGrammar α V T) :
+    (Mapped f E).initialWord = mapWord f E.initialWord := rfl
+
+@[simp]
+lemma mapped_rewriteWord {α α' V T} (f : α → α') (E : EDT0LGrammar α V T) (t : T) (w) :
+    (E.Mapped f).rewriteWord t (mapWord f w) = mapWord f (E.rewriteWord t w) := by
+  induction w with
+  | nil =>
+    rfl
+  | cons x xs ih =>
+    simp only [mapWord_cons, rewriteWord_cons, ih, mapWord_append, List.append_cancel_right_eq]
+    split <;> rfl
+
+@[simp]
+lemma mapped_rewriteSeq {α α' V T} (f : α → α') (E : EDT0LGrammar α V T) (s : List T) (w) :
+    (E.Mapped f).rewriteSeq s (mapWord f w) = mapWord f (E.rewriteSeq s w) := by
+  induction s using List.reverseRecOn with
+  | nil => rfl
+  | append_singleton xs x ih => simp [ih]
+
+lemma mapped_language {α α' V T} (f : α → α') (E : EDT0LGrammar α V T) :
+    (E.Mapped f).language = E.language.map f := by
+  ext1 w
+  simp only [language_mem_iff, generates_iff_rewriteSeq, mapped_initialWord, mapped_rewriteSeq]
+  constructor
+  · intro h
+    obtain ⟨s, h⟩ := h
+    obtain ⟨u, h'⟩ := mapWord_eq_terminals _ _ _ h
+    use u
+    constructor
+    · simp only [language, Set.mem_setOf_eq, ← h']
+      exact generates_rewriteSeq E
+    · rw [h', mapWord_terminals] at h
+      change List.map (Symbol.terminal ∘ f) _ = _ at h
+      rw [← List.map_map (f := f) (g := (Symbol.terminal (T := α') (N := V))) (l := u)] at h
+      simp only [List.map_terminal] at h
+      exact h
+  · intro h
+    obtain ⟨w', h1, h2⟩ := h
+    simp only [language, generates_iff_rewriteSeq, Set.mem_setOf_eq] at h1
+    obtain ⟨s, h1⟩ := h1
+    use s
+    rw [h1]
+    simp only [mapWord_terminals]
+    change List.map (Symbol.terminal ∘ f) _ = _
+    rw [← List.map_map (f := f) (g := (Symbol.terminal (T := α') (N := V))) (l := w')]
+    simp only [List.map_terminal]
+    exact h2
+
+end EDT0LGrammar
+
+lemma Language.isEDT0L_map {α α'} (f : α → α') (L : Language α) (h : L.IsEDT0L) :
+    (L.map f).IsEDT0L := by
+  obtain ⟨n, m, E, h⟩ := h
+  use n, m, E.Mapped f
+  subst h
+  exact EDT0LGrammar.mapped_language f E
+
