LSystems/EDT0L/RewriteSequence.lean
@@ -1,0 +1,208 @@
+/-
+Copyright (c) 2025 Alex Bishop. All rights reserved.
+Released under Apache 2.0 license as described in the file LICENSE.
+Author: Alex Bishop
+-/
+module
+
+public import LSystems.EDT0L.Defs
+
+/-!
+# Sequences of rewrites
+
+Suppsose that `E : EDT0LGrammar α V T`, and that `u v : List (Symbol α V)` are two words.  Then,
+from the definitions provided in `LSystems.EDT0l.Defs`, we see that `E.Derives u v` if and only if
+there exists some sequence of tables which can be used to rewrite `u` to `v`.  In this file, we give
+an alternative definition which makes this sequence of tables explicit.
+
+## Main definition
+
+* `EDT0LGrammar.rewriteSeq E s w`: the word that would be obtained by applying the tables in `s` to
+  the word `w` in order.  (see this definition for more details.)
+
+## Main theorem
+
+* `EDT0LGrammar.derives_iff_rewriteSeq`: shows that, in some way, `EDT0LGrammar.Derives` and
+  `EDT0LGrammar.rewriteSeq` are equivelent.
+-/
+
+@[expose] public section
+
+namespace EDT0LGrammar
+variable {α V T} (E : EDT0LGrammar α V T)
+
+/--
+Suppose that $s = [s_1, s_2, ..., s_k]$ is a sequence of tables, and that $w$ is some word.  Then,
+we may define a sequence of words $w_1, w_2, ..., w_k$ where $w_1$ is the word `E.rewriteWord s₁ w`,
+and $w_{i+1}$ is the word `E.rewriteWord sᵢ wᵢ` for each $i \in \{ 1,2,...,k - 1 \}$.  We then
+define `E.rewriteSeq s w` to be the word $w_k$, that is, the word obtained by applying the sequence
+of tables $s$ to the word $w$.
+
+This definition is important for the definition of the class of LULT EDT0L grammars as defined in
+`LSystems.FiniteIndexEDT0L.LULT`.
+-/
+def rewriteSeq (s : List T) (w : List (Symbol α V)) : List (Symbol α V) :=
+  List.foldl (fun w' τ ↦ E.rewriteWord τ w') w s
+
+@[simp]
+lemma rewriteSeq_refl (w : List (Symbol α V)) : E.rewriteSeq [] w = w := rfl
+
+@[simp]
+lemma rewriteSeq_nil (s : List T) : E.rewriteSeq s [] = [] := List.foldl_fixed' (congrFun rfl) s
+
+@[simp]
+lemma rewriteSeq_seq_single (t : T) (w : List (Symbol α V)) :
+    E.rewriteSeq [t] w = E.rewriteWord t w := rfl
+
+@[simp]
+lemma rewriteSeq_seq_append_singleton {t : T} {ts : List T} {u : List (Symbol α V)} :
+    E.rewriteSeq (ts ++ [t]) u = E.rewriteWord t (E.rewriteSeq ts u) := List.foldl_concat _ u t ts
+
+@[simp]
+lemma rewriteSeq_seq_cons {t : T} {ts : List T} {u : List (Symbol α V)} :
+    E.rewriteSeq (t::ts) u = E.rewriteSeq ts (E.rewriteWord t u) := List.foldl_cons
+
+@[simp]
+lemma rewriteSeq_seq_append (t s w) :
+    E.rewriteSeq (s ++ t) w = E.rewriteSeq t (E.rewriteSeq s w) := List.foldl_append
+
+@[simp]
+lemma rewriteSeq_append (s : List T) (u v : List (Symbol α V)) :
+    E.rewriteSeq s (u ++ v) = E.rewriteSeq s u ++ E.rewriteSeq s v := by
+  induction s using List.reverseRec with
+  | nil => rfl
+  | append_singleton xs x ih => simp [ih]
+
+lemma rewriteSeq_cons (s : List T) (a : Symbol α V) (as : List (Symbol α V)) :
+    E.rewriteSeq s (a::as) = E.rewriteSeq s [a] ++ E.rewriteSeq s as := by
+  rw [← rewriteSeq_append]
+  simp only [List.cons_append, List.nil_append]
+
+@[simp]
+lemma rewriteSeq_terminals {s : List T} {u : List α} :
+    E.rewriteSeq s (u.map .terminal) = u.map .terminal := by
+  induction s using List.reverseRecOn with
+  | nil => rfl
+  | append_singleton xs x ih => simp [ih]
+
+@[simp]
+lemma rewriteSeq_terminal {s : List T} {u : α} :
+    E.rewriteSeq s [.terminal u] = [.terminal u] := by
+  induction s using List.reverseRecOn with
+  | nil => rfl
+  | append_singleton xs x ih => simp [ih]
+
+theorem derives_iff_rewriteSeq (w w' : List (Symbol α V)) :
+    E.Derives w w' ↔ ∃ s : List T, E.rewriteSeq s w = w' := by
+  constructor
+  · intro h
+    induction h with
+    | refl =>
+      use []
+      rfl
+    | tail x y z =>
+      rename_i a b
+      obtain ⟨s, rfl⟩ := z
+      obtain ⟨t, rfl⟩ := y
+      exact ⟨s ++ [t], E.rewriteSeq_seq_append_singleton⟩
+  · intro h
+    obtain ⟨s, rfl⟩ := h
+    induction s using List.reverseRecOn with
+    | nil =>
+      simp only [rewriteSeq_refl]
+      exact derives_refl
+    | append_singleton xs x ih =>
+      simp only [rewriteSeq_seq_append, rewriteSeq_seq_cons, rewriteSeq_refl]
+      exact derives_tail' ih x
+
+theorem generates_iff_rewriteSeq (w : List (Symbol α V)) :
+    E.Generates w ↔ ∃ s : List T, E.rewriteSeq s E.initialWord = w := by
+  constructor
+  · intro h
+    induction h with
+    | refl =>
+      use []
+      rfl
+    | tail x y ih =>
+      rename_i a b
+      obtain ⟨s, rfl⟩ := ih
+      obtain ⟨t, rfl⟩ := y
+      use s ++ [t]
+      simp
+  · intro h
+    obtain ⟨s, rfl⟩ := h
+    induction s using List.reverseRecOn with
+    | nil =>
+      simp only [rewriteSeq_refl]
+      exact generates_initial E
+    | append_singleton xs x ih =>
+      simp only [rewriteSeq_seq_append, rewriteSeq_seq_cons, rewriteSeq_refl]
+      exact generates_rewriteWord_tail ih x
+
+lemma generates_rewriteSeq {s : List T} : E.Generates (E.rewriteSeq s E.initialWord) := by
+  simp [generates_iff_rewriteSeq]
+
+lemma derives_rewriteSeq {s : List T} {w : List (Symbol α V)} : E.Derives w (E.rewriteSeq s w) := by
+  simp [derives_iff_rewriteSeq]
+
+@[simp]
+lemma equiv_rewriteSeq {α' V' T'}
+  (equivα : α ≃ α') (equivV : V ≃ V') (equivT : T ≃ T')
+  (t : List T)
+  (u : List (Symbol α V)) :
+    ((equiv equivα equivV equivT E).rewriteSeq (t.map equivT) (equivWord equivα equivV u)) =
+      equivWord equivα equivV (E.rewriteSeq t u) := by
+  induction t using List.reverseRecOn with
+  | nil => rfl
+  | append_singleton xs x ih => simp [ih]
+
+@[simp]
+lemma equiv_rewriteSeq' {α' V' T'}
+  (equivα : α ≃ α') (equivV : V ≃ V') (equivT : T ≃ T')
+  (t : List T')
+  (u : List (Symbol α' V')) :
+    ((equiv equivα equivV equivT E).rewriteSeq t u) =
+      equivWord equivα equivV (E.rewriteSeq (t.map equivT.symm)
+        (equivWord equivα.symm equivV.symm u)) := by
+  have := E.equiv_rewriteSeq equivα equivV equivT
+    (t.map equivT.symm) (equivWord equivα.symm equivV.symm u)
+  simpa
+
+-- @[simp]
+-- lemma rewriteSeq_count_equivWord {α' V' T'}
+--   [DecidableEq α] [DecidableEq V]
+--   [DecidableEq α'] [DecidableEq V']
+--   (equivα : α ≃ α') (equivV : V ≃ V') (equivT : T ≃ T')
+--   (t : List T)
+--   (u : List (Symbol α V)) (s : Symbol α V) :
+--     List.count
+--       (equivSymbol equivα equivV s)
+--       ((equiv equivα equivV equivT E).rewriteSeq
+--         (t.map equivT)
+--         (equivWord equivα equivV u)) =
+--     List.count s (E.rewriteSeq t u) := by
+--   simp only [rewriteSeq_equivWord]
+--   induction (E.rewriteSeq t u) with
+--   | nil =>
+--     rfl
+--   | cons x xs ih =>
+--     simp only [equivWord_cons, List.count_cons, ih, beq_iff_eq, EmbeddingLike.apply_eq_iff_eq]
+--
+-- @[simp]
+-- lemma rewriteSeq_length_equivWord {α' V' T'}
+--   (equivα : α ≃ α') (equivV : V ≃ V') (equivT : T ≃ T')
+--   (t : List T)
+--   (u : List (Symbol α V)) :
+--     List.length
+--       ((equiv equivα equivV equivT E).rewriteSeq
+--         (t.map equivT)
+--         (equivWord equivα equivV u)) =
+--     List.length (E.rewriteSeq t u) := by
+--   simp only [rewriteSeq_equivWord]
+--   induction (E.rewriteSeq t u) with
+--   | nil =>
+--     rfl
+--   | cons x xs ih =>
+--     simp only [equivWord_cons, List.length_cons, ih]
+
+end EDT0LGrammar
