LSystems/FiniteIndexEDT0L.lean
@@ -1,9 +1,11 @@
 /-
 Copyright (c) 2025 Alex Bishop. All rights reserved.
 Released under Apache 2.0 license as described in the file LICENSE.
-Author: Alex Bishop
+Authors: Alex Bishop
 -/
+import LSystems.FiniteIndexEDT0L.Attach
 import LSystems.FiniteIndexEDT0L.Defs
 import LSystems.FiniteIndexEDT0L.LULT
+import LSystems.FiniteIndexEDT0L.Mapped
 import LSystems.FiniteIndexEDT0L.RegularLanguage
 import LSystems.FiniteIndexEDT0L.Union
