LSystems/FiniteIndexEDT0L/Attach.lean
@@ -1,0 +1,55 @@
+/-
+Copyright (c) 2026 Alex Bishop. All rights reserved.
+Released under Apache 2.0 license as described in the file LICENSE.
+Author: Alex Bishop
+-/
+module
+
+public import LSystems.EDT0L.Attach
+public import LSystems.FiniteIndexEDT0L.Defs
+
+@[expose] public section
+
+namespace EDT0LGrammar
+
+lemma attach_isIndex {α V T} [BEq V] (E : EDT0LGrammar α V T) {k : ℕ} (h : E.IsIndex k) :
+    E.attach.IsIndex k := by
+  intro w hw
+  have := h (unattachSymbolWord w) (by
+    simp_all only [generates_iff_rewriteSeq]
+    obtain ⟨s, rfl⟩ := hw
+    use s
+    rw [attach_rewriteSeq (h := Eq.symm (unattachSymbolWord_initialWord (E := E)))] )
+  simp_all
+
+lemma attach_isIndex' {α V T} [BEq V] (E : EDT0LGrammar α V T) {k : ℕ} (h : E.attach.IsIndex k) :
+    E.IsIndex k := by
+  intro w hw
+  rw [generates_iff_rewriteSeq] at hw
+  obtain ⟨s, hw⟩ := hw
+  rw [attach_rewriteSeq (h := Eq.symm unattachSymbolWord_initialWord)] at hw
+  change let w' := _ ;  unattachSymbolWord  w' = _ at hw
+  extract_lets w' at hw
+  subst hw
+  have := h w' (by
+    subst w'
+    exact generates_rewriteSeq E.attach )
+  simp_all
+
+lemma attach_isIndex_iff {α V T} [BEq V] (E : EDT0LGrammar α V T) {k : ℕ} :
+    E.attach.IsIndex k ↔ E.IsIndex k := ⟨attach_isIndex' E, attach_isIndex E⟩
+
+lemma attach_isFiniteIndex_iff {α V T} [BEq V] (E : EDT0LGrammar α V T) :
+    E.attach.IsFiniteIndex ↔ E.IsFiniteIndex := by
+  constructor
+  · intro h
+    obtain ⟨k, h⟩ := h
+    rw [attach_isIndex_iff] at h
+    exact ⟨_, h⟩
+  · intro h
+    obtain ⟨k, h⟩ := h
+    rw [<- attach_isIndex_iff] at h
+    exact ⟨_, h⟩
+
+end EDT0LGrammar
+
