LSystems/FiniteIndexEDT0L/LULT/Attach.lean
@@ -1,0 +1,64 @@
+/-
+Copyright (c) 2026 Alex Bishop. All rights reserved.
+Released under Apache 2.0 license as described in the file LICENSE.
+Author: Alex Bishop
+-/
+module
+
+public import LSystems.EDT0L.Attach
+public import LSystems.FiniteIndexEDT0L.LULT.Defs
+
+@[expose] public section
+
+namespace EDT0LGrammar
+
+lemma attach_isLULT {α V T} [BEq V] (E : EDT0LGrammar α V T) (h : E.IsLULT) : E.attach.IsLULT := by
+  intro w hw
+  obtain ⟨s, h1, h2⟩ := h w.unattach (by 
+    rw [← language_eq_attach_language_map_val]
+    use w, hw
+    simp)
+  use s
+  constructor
+  · rw [attach_rewriteSeq (h := Eq.symm (unattachSymbolWord_initialWord (E := E)))] at h1
+    refine unattachSymbolWord_congr ?_
+    rw [h1]
+    simp
+  · intro v i hi
+    replace h2 := h2 v i hi
+    obtain h2 | h2 := h2
+    · left
+      rw [attach_rewriteSeq (h := Eq.symm (unattachSymbolWord_initialWord (E := E)))] at h2
+      simp only [filterNonterminals_unattachSymbolWord] at h2
+      exact h2
+    · right
+      rw [attach_rewriteSeq (w := [.nonterminal v]) (w' := [.nonterminal v]) (h := rfl)] at h2
+      unfold unattachSymbolWord at h2
+      simpa using h2
+
+lemma attach_isLULT_iff {α V T} [BEq V] (E : EDT0LGrammar α V T) : E.attach.IsLULT ↔ E.IsLULT := by
+  classical
+  constructor
+  · intro h w hw
+    rw [← language_eq_attach_language_map_val] at hw
+    obtain ⟨w', hw', h'⟩ := hw
+    replace ⟨s, h1, h2⟩ := h w' hw'
+    use s
+    constructor
+    · clear * - h1 h'
+      subst h'
+      simp only [forall_exists_index, List.map_subtype, List.map_id_fun', id_eq]
+      rw [attach_rewriteSeq (h := Eq.symm (unattachSymbolWord_initialWord (E := E)))]
+      rw [h1]
+      simp
+    · intro v i hi
+      obtain h2 | h2 := h2 v i hi
+      · left
+        rw [attach_rewriteSeq (h := Eq.symm (unattachSymbolWord_initialWord (E := E)))]
+        simp_all
+      · right
+        rw [attach_rewriteSeq (w := [.nonterminal v]) (w' := [.nonterminal v]) (h := rfl)]
+        simp_all
+  · exact attach_isLULT E
+
+end EDT0LGrammar
