LSystems/FiniteIndexEDT0L/LULT/Basic.lean
@@ -3,30 +3,18 @@ Copyright (c) 2025 Alex Bishop. All rights reserved.
 Released under Apache 2.0 license as described in the file LICENSE.
 Author: Alex Bishop
 -/
-import LSystems.FiniteIndexEDT0L.Defs
-import LSystems.FiniteIndexEDT0L.LULT.Defs
-import LSystems.FiniteIndexEDT0L.LULT.LULTImpFiEDT0L.Defs
-import LSystems.FiniteIndexEDT0L.LULT.LULTImpFiEDT0L.Generates
+module
 
-namespace EDT0LGrammar
+public import LSystems.FiniteIndexEDT0L.Defs
+public import LSystems.FiniteIndexEDT0L.LULT.Defs
 
-lemma lult_imp_fiedt0l {α} (L : Language α) :
-    L.IsLULT → L.IsFiniteIndexEDT0L := by
-  intro h
-  obtain ⟨n,m,E,h,h'⟩ := h
-  classical
-  let E' := LULTImpFiEDT0L E
-  have h₁ : E.language = E'.language := by
-    unfold E' EDT0LGrammar.language
-    simp only [LULTImpFiEDT0L.generates_iff, h]
-  rw [h₁] at h'
-  rw [← h']
-  have h₂ := LULTImpFiEDT0L.finite_index E
-  change E'.IsIndex _ at h₂
-  simp only [Fintype.card_fin] at h₂
-  use n + 1
-  exact fi_edt0l_grammars_generate_fi_edt0l_languages' E' h₂
+import LSystems.FiniteIndexEDT0L.LULT.LULTImpFiEDT0L
+import LSystems.FiniteIndexEDT0L.LULT.FiEDT0LImpLULT
 
-end EDT0LGrammar
+@[expose] public section
 
+@[simp]
+theorem Language.isLULT_iff_isFiniteIndexEDT0L {α} (L : Language α) :
+    L.IsLULT ↔ L.IsFiniteIndexEDT0L :=
+  ⟨L.isLULT_imp_isFiniteIndexEDT0L, L.isFiniteIndexEDT0L_imp_isLULT⟩
 
