LSystems/FiniteIndexEDT0L/LULT/FiEDT0LImpLULT.lean
@@ -1,0 +1,1078 @@
+/-
+Copyright (c) 2025 Alex Bishop. All rights reserved.
+Released under Apache 2.0 license as described in the file LICENSE.
+Author: Alex Bishop
+-/
+module
+
+public import LSystems.FiniteIndexEDT0L.Defs
+public import LSystems.FiniteIndexEDT0L.LULT.Defs
+public import Mathlib.Data.Finset.Lattice.Fold
+public import Mathlib.Data.Fintype.Pi
+
+import Mathlib.Data.Fin.Tuple.Take
+
+@[expose] public section
+
+namespace EDT0LGrammar
+namespace FiEDT0L2LULT
+
+structure Word (V : Type*) (k : ℕ) where
+  ℓ : Fin (k + 1)
+  get : Fin ℓ → V
+deriving DecidableEq
+
+instance (V : Type*) [Fintype V] [DecidableEq V] (k : ℕ) :
+    Fintype (Word V k) where
+  elems :=
+    Fintype.elems.sup fun (ℓ : Fin (k + 1)) ↦
+    Fintype.elems.sup fun (word : Fin ℓ → V) ↦
+    {⟨ℓ, word⟩}
+  complete := by
+    intro x
+    simp only [Finset.sup_singleton_apply, Finset.mem_sup, Finset.mem_image]
+    exact ⟨x.ℓ, Fintype.complete _, x.get, Fintype.complete _, rfl⟩
+
+structure Nonterminal (V : Type*) (k : ℕ) where
+  word : Word V k
+  i : Fin word.ℓ
+deriving DecidableEq
+
+instance (V : Type*) [Fintype V] [DecidableEq V] (k : ℕ) :
+    Fintype (Nonterminal V k) where
+  elems :=
+    Fintype.elems.sup fun (word : Word V k) ↦
+    Fintype.elems.sup fun (i : Fin word.ℓ) ↦
+    {⟨word, i⟩}
+  complete := by
+    intro x
+    simp only [Finset.sup_singleton_apply, Finset.mem_sup, Finset.mem_image]
+    exact ⟨x.word, Fintype.complete _, x.i, Fintype.complete _, rfl⟩
+
+namespace Nonterminal
+
+def unlabel {V k} (v : Nonterminal V k) := v.word.get v.i
+
+end Nonterminal
+
+-- -----------------------
+
+namespace Word
+
+def mk' {α V k}
+  {w : List (Symbol α V)}
+  (h : List.length (filterNonterminals w) ≤ k) :
+    Word V k where
+  ℓ := ⟨List.length (filterNonterminals w), Nat.lt_succ_of_le h⟩
+  get := (filterNonterminals w).get
+
+def toList {V k} (v : Word V k) := List.ofFn v.get
+
+def toNumberedList {V k} (v : Word V k) : List (Nonterminal V k) :=
+  List.ofFn fun i ↦ ⟨v, i⟩
+
+@[simp]
+lemma mk'_toList {α V k}
+  {w : List (Symbol α V)}
+  (h : List.length (filterNonterminals w) ≤ k) :
+    (mk' h).toList = filterNonterminals w := List.ofFn_get (filterNonterminals w)
+
+lemma toNumberedList_nodup {V k} (v : Word V k) : v.toNumberedList.Nodup := by
+  unfold toNumberedList
+  rw [List.nodup_iff_pairwise_ne]
+  rw [List.pairwise_ofFn]
+  simp only [ne_eq, Nonterminal.mk.injEq, heq_eq_eq, true_and]
+  exact fun ⦃i j⦄ a ↦ Fin.ne_of_lt a
+
+lemma toList_length {V k} (v : Word V k) : v.toList.length = v.ℓ := by simp [toList]
+
+def rewriteFilterNonterminals {α V T k} (v : Word V k) (E : EDT0LGrammar α V T) (t : T) :
+    List V := filterNonterminals (List.flatMap (E.table t) v.toList)
+
+def rewriteFilterNonterminalsTake {α V T k} (v : Word V k) (E : EDT0LGrammar α V T) (t : T)
+  (i : ℕ) : List V := filterNonterminals (List.flatMap (E.table t) (v.toList.take i))
+
+def rewriteFilterNonterminalsGet {α V T k} (v : Word V k) (E : EDT0LGrammar α V T) (t : T)
+  (i : Fin v.ℓ) : List V := filterNonterminals (E.table t (v.get i))
+
+def rewriteLength {α V T k} (v : Word V k) (E : EDT0LGrammar α V T) (t : T) : ℕ :=
+  List.length <| v.rewriteFilterNonterminals E t
+
+def CanRewrite {α V T k} (v : Word V k) (E : EDT0LGrammar α V T) (t : T) : Prop :=
+   v.rewriteLength E t < k + 1
+
+variable {α V T k} (v : Word V k) (E : EDT0LGrammar α V T) (t : T) in
+instance : Decidable (v.CanRewrite E t) := by
+  unfold CanRewrite
+  exact inferInstance
+
+lemma canRewrite_rewriteSeq {α V T} (E : EDT0LGrammar α V T) {k} (h : E.IsIndex k)
+  (xs : List T) (x : T) :
+    (Word.mk'
+        (w := E.rewriteSeq xs E.initialWord)
+        (h _ E.generates_rewriteSeq)).CanRewrite E x := by
+  simp only [Word.CanRewrite, Word.rewriteLength,
+    Word.rewriteFilterNonterminals, Word.mk'_toList]
+  rw [← filterNonterminals_rewriteSymbols, ← rewriteSeq_seq_append_singleton]
+  rw [← Nat.le_iff_lt_add_one]
+  exact h _ E.generates_rewriteSeq
+
+def rewrite {α V T k} (v : Word V k) (E : EDT0LGrammar α V T) (t : T) (h : v.CanRewrite E t) :
+    Word V k where
+  ℓ := ⟨v.rewriteLength E t, h⟩
+  get := (v.rewriteFilterNonterminals E t).get
+
+def numberNonterminals {α V k} (target : Word V k) :
+    (w : List (Symbol α V)) →
+    (i : ℕ) → (j : ℕ) →
+    (h : filterNonterminals w = (target.toList.drop i).take j) →
+    (h' : (filterNonterminals w).length = j) →
+    List (Symbol α (Nonterminal V k))
+  | [],_,_,_,_ => []
+  | .terminal x::xs, i, j, h, h' =>
+    .terminal x :: target.numberNonterminals xs i j (by simpa using h) (by simpa using h')
+  | .nonterminal x::xs, i, j, h, h' =>
+    .nonterminal ⟨target, ⟨i, by
+      by_contra contra
+      rw [← toList_length] at contra
+      simp only [not_lt] at contra
+      simp [List.drop_of_length_le contra] at h⟩⟩ ::
+    target.numberNonterminals xs (i + 1) (j - 1) (by
+      simp only [filterNonterminals_cons] at h
+      cases j with
+      | zero =>
+        simp at h
+      | succ m =>
+        rw [Nat.add_comm m 1, List.take_add, List.take_one] at h
+        unfold List.head? at h
+        split at h
+        · rename_i heq
+          rw [heq] at h
+          simp at h
+        · rename_i a as heq
+          simp only [Option.toList_some, List.drop_drop, List.cons_append, List.nil_append,
+            List.cons.injEq] at h
+          obtain ⟨rfl, h⟩ := h
+          simpa using h)
+      (by cases j with | zero => simp at h' | succ j' => simpa using h' )
+
+def rewriteNonterminal {α V T k} (v : Word V k) (E : EDT0LGrammar α V T) (t : T)
+  (h : v.CanRewrite E t) (i : Fin v.ℓ) :
+    List (Symbol α (Nonterminal V k)) :=
+  (v.rewrite E t h).numberNonterminals
+    (E.table t (v.get i))
+    (List.length <| v.rewriteFilterNonterminalsTake E t i)
+    (List.length <| v.rewriteFilterNonterminalsGet E t i)
+    (by
+      unfold rewriteFilterNonterminalsTake rewriteFilterNonterminalsGet
+      conv => rhs; arg 2; arg 2; unfold Word.rewrite Word.toList
+      simp only
+      unfold Word.rewriteFilterNonterminals
+      --
+      change let s := _; _ = List.take _ (List.drop _ s)
+      intro s
+      have : s = filterNonterminals (List.flatMap (E.table t) v.toList) := List.ofFn_get _
+      rw [this]
+      clear this
+      --
+      conv => rhs; arg 2; arg 2; rw [← List.take_append_drop (↑i) v.toList]
+      rw [List.flatMap_append, filterNonterminals_append]
+      simp only [List.drop_left']
+      have : List.drop (↑i) v.toList = v.toList.get ⟨i, by simp [toList_length]⟩ ::
+          List.drop (↑i + 1) v.toList := Eq.symm List.cons_get_drop_succ
+      rw [this]
+      clear this
+      --
+      rw [List.flatMap_cons, filterNonterminals_append]
+      conv => rhs; arg 2; lhs; unfold Word.toList
+      simp )
+    rfl
+
+end Word
+
+-- -----------------------
+
+namespace Nonterminal
+
+def letter {V k} (v : Nonterminal V k) : V := v.word.get v.i
+
+def rewrite {α V T k} (v : Nonterminal V k) (E : EDT0LGrammar α V T) (t : T)
+  (h : v.word.CanRewrite E t) :
+    List (Symbol α (Nonterminal V k)) := v.word.rewriteNonterminal E t h v.i
+
+end Nonterminal
+
+-- -----------------------
+
+def UnlabelWord {α V} {k : ℕ}
+  (w : List (Symbol α (Nonterminal V k))) :
+    List (Symbol α V) :=
+  w.map
+    (fun
+      | .terminal a => .terminal a
+      | .nonterminal v => .nonterminal v.letter)
+
+@[simp]
+lemma unlabelWord_append {α V} {k : ℕ}
+  (u v : List (Symbol α (Nonterminal V k))) :
+    UnlabelWord (u ++ v) = UnlabelWord u ++ UnlabelWord v := List.map_append
+
+@[simp]
+lemma unlabelWord_cons {α V} {k : ℕ}
+  (a : Symbol α (Nonterminal V k)) (as : List (Symbol α (Nonterminal V k))) :
+    UnlabelWord (a::as) =
+    (match a with
+      | .terminal a => .terminal a
+      | .nonterminal v => .nonterminal v.letter)
+    :: UnlabelWord as := List.map_cons
+
+@[simp]
+lemma unlabelWord_nil {α V} {k : ℕ} : UnlabelWord (α := α) (V := V) (k := k) [] = [] := rfl
+
+@[simp]
+lemma unlabelWord_length {α V k} (w : List (Symbol α (Nonterminal V k))) :
+    (UnlabelWord w).length = w.length := by simp [UnlabelWord]
+
+@[simp]
+lemma unlabelWord_numberNonterminals {α V k} (target : Word V k)
+  (w : List (Symbol α V))
+  (i j : ℕ)
+  (h : filterNonterminals w = (target.toList.drop i).take j)
+  (h' : (filterNonterminals w).length = j) :
+    UnlabelWord (target.numberNonterminals w i j h h') = w := by
+  let rec go : 
+      (w : List (Symbol α V)) →
+      (i j : ℕ) →
+      (h : filterNonterminals w = (target.toList.drop i).take j) →
+      (h' : (filterNonterminals w).length = j) →
+        UnlabelWord (target.numberNonterminals w i j h h') = w
+    | [],_,_,_,_ => rfl
+    | a::as,i,j,h',h'' => by
+      cases a with
+      | terminal a =>
+        unfold Word.numberNonterminals
+        simp only [unlabelWord_cons, List.cons.injEq, true_and]
+        simp only [filterNonterminals_cons] at h'
+        exact go as i j h' h''
+      | nonterminal v =>
+        unfold Word.numberNonterminals
+        simp only [unlabelWord_cons, List.cons.injEq, Symbol.nonterminal.injEq]
+        simp only [filterNonterminals_cons] at h'
+        cases j with
+        | zero =>
+          simp at h'
+        | succ j' =>
+          rw [Nat.add_comm, List.take_add] at h'
+          cases hl : List.drop i target.toList with
+          | nil =>
+            simp [hl] at h'
+          | cons b bs =>
+            simp only [hl, List.take_succ_cons, List.take_zero, List.drop_succ_cons, List.drop_zero,
+              List.cons_append, List.nil_append, List.cons.injEq] at h'
+            obtain ⟨rfl, h'⟩ := h'
+            constructor
+            · unfold Nonterminal.letter
+              simp only
+              replace hl := congrArg List.head? hl
+              simp only [Word.toList, List.head?_drop, List.getElem?_ofFn, List.head?_cons,
+                Option.dite_none_right_eq_some, Option.some.injEq] at hl
+              obtain ⟨h, hl⟩ := hl
+              exact hl
+            · replace hl := congrArg (List.drop 1) hl
+              simp only [List.drop_drop, List.drop_succ_cons, List.drop_zero] at hl
+              subst hl
+              simp only [Nat.add_one_sub_one]
+              exact go _ _ _ h' (by
+                clear * - h''
+                simp only [filterNonterminals_cons, List.length_cons,
+                  Nat.add_right_cancel_iff] at h''
+                omega )
+  exact go _ _ _ _ _
+
+@[simp]
+lemma Word.numberNonterminals_eq_nil {α V k} (target : Word V k)
+  (w : List (Symbol α V))
+  (i : ℕ)
+  (h : filterNonterminals w = (target.toList.drop i).take 0)
+  (h' : (filterNonterminals w).length = 0) :
+    filterNonterminals (target.numberNonterminals w i 0 h h') = [] := by
+  rw [List.eq_nil_iff_length_eq_zero]
+  induction w with
+  | nil =>
+    rfl
+  | cons x xs ih =>
+    simp only [List.take_zero, List.length_eq_zero_iff, Subsingleton.forall₂_iff] at ih ⊢
+    replace ih := ih (by
+      simp only [filterNonterminals_cons, List.length_eq_zero_iff] at h'
+      split at h' <;> simp_all )
+    unfold numberNonterminals
+    cases x with
+    | terminal a => simp_all
+    | nonterminal v => simp at h'
+
+@[simp]
+lemma list_append_eq_list_take_append {α} {u v x y : List α} :
+    u ++ v = x.take u.length ++ y.take v.length ↔ u = x.take u.length ∧ v = y.take v.length := by
+  constructor
+  · intro h
+    if huv : u.length ≤ x.length ∧ v.length ≤ y.length then
+      constructor
+      · replace h := congrArg (List.take u.length) h
+        simp only [List.take_left', List.length_take, huv, inf_of_le_left] at h
+        exact h
+      · replace h := congrArg (List.drop u.length) h
+        simp only [List.drop_left', List.length_take, huv, inf_of_le_left] at h
+        exact h
+    else
+      exfalso
+      simp only [not_and_or, not_le] at huv
+      obtain hu | hv := huv
+      · replace h := congrArg List.length h
+        simp [min_eq_right (show x.length ≤ u.length by omega)] at h
+        omega
+      · replace h := congrArg List.length h
+        simp [min_eq_right (show y.length ≤ v.length by omega)] at h
+        omega
+  · intro h
+    conv => lhs ; rw [h.left, h.right]
+
+@[simp]
+lemma Word.numberNonterminals_nil {α V k} (target : Word V k)
+  (i j : ℕ)
+  (h : filterNonterminals (α := α) (V := V) [] = (target.toList.drop i).take j)
+  (h' : (filterNonterminals (α := α) (V := V) []).length = j) :
+    target.numberNonterminals [] i j h h' = [] := rfl
+
+@[simp]
+lemma Word.numberNonterminals_append {α V k} (target : Word V k)
+  (u v : List (Symbol α V))
+  (i j : ℕ)
+  (h : filterNonterminals (u ++ v) = (target.toList.drop i).take j)
+  (h' : (filterNonterminals (u ++ v)).length = j) :
+    target.numberNonterminals (u ++ v) i j h h' =
+      target.numberNonterminals u i
+        (filterNonterminals u).length
+        (by
+          simp only [filterNonterminals_append, List.length_append] at h'
+          subst h'
+          simp only [filterNonterminals_append] at h
+          rw [List.take_add] at h
+          simp only [List.drop_drop, list_append_eq_list_take_append] at h
+          rw [h.left]
+          simp)
+        rfl ++
+      target.numberNonterminals v (i + (filterNonterminals u).length)
+        (filterNonterminals v).length
+        (by
+          simp only [filterNonterminals_append, List.length_append] at h'
+          subst h'
+          simp only [filterNonterminals_append] at h
+          rw [List.take_add] at h
+          simp only [List.drop_drop, list_append_eq_list_take_append] at h
+          rw [h.right]
+          simp)
+        rfl := by
+  induction u generalizing i j with
+  | nil =>
+    subst h'
+    simp_all
+  | cons x xs ih =>
+    subst h'
+    cases x with
+    | terminal a =>
+      conv =>
+        lhs
+        arg 2
+        rw [List.cons_append (a := .terminal a) (as := xs) (bs := v)]
+      rw [numberNonterminals]
+      conv =>
+        lhs
+        rhs
+        simp only [List.cons_append, filterNonterminals_cons]
+      --
+      replace ih := ih i (filterNonterminals (xs ++ v)).length (by simp_all) rfl
+      rw [ih]
+      rfl
+    | nonterminal n =>
+      conv =>
+        lhs
+        arg 2
+        rw [List.cons_append (a := .nonterminal n) (as := xs) (bs := v)]
+      rw [numberNonterminals]
+      conv =>
+        lhs
+        rhs
+        tactic => simp only [List.cons_append, filterNonterminals_cons,
+          List.length_cons, Nat.add_one_sub_one]
+      --
+      replace ih := ih (i + 1) (filterNonterminals (xs ++ v)).length
+        (by
+          refine (List.cons_inj_right n).mp ?_
+          rw [List.cons_append (a := .nonterminal n) (as := xs) (bs := v)] at h
+          conv at h =>
+            lhs
+            simp only [filterNonterminals_cons]
+          rw [h]
+          have h' :
+            (n :: filterNonterminals (xs ++ v))[0]? =
+            (List.take (filterNonterminals (Symbol.nonterminal n :: (xs ++ v))).length
+              (List.drop i target.toList))[0]? := by rw [h]
+          simp only [filterNonterminals_append, List.length_cons, List.length_append,
+            Nat.zero_lt_succ, getElem?_pos, List.getElem_cons_zero, filterNonterminals_cons,
+            List.getElem?_take_of_lt, List.getElem?_drop, add_zero] at h'
+          --
+          simp only [filterNonterminals_cons, List.length_cons]
+          rw [Nat.add_comm _ 1, List.take_add, ← List.singleton_append, List.drop_drop]
+          rw [List.append_cancel_right_eq]
+          clear * - h'
+          rw [List.some_eq_getElem?_iff] at h'
+          obtain ⟨h, rfl⟩ := h'
+          rw [List.take_one_drop_eq_of_lt_length h]
+          rfl )
+        rfl
+      rw [ih]
+      conv => rhs ; rw [numberNonterminals]
+      simp only [filterNonterminals_cons, List.length_cons, Nat.add_one_sub_one, List.cons_append,
+        List.cons.injEq, List.append_cancel_left_eq, true_and]
+      simp only [Nat.add_comm (filterNonterminals xs).length 1, Nat.add_assoc]
+
+@[simp]
+lemma Word.numberNonterminals_length {α V k} (target : Word V k)
+  (u : List (Symbol α V))
+  (i j : ℕ)
+  (h : filterNonterminals u = (target.toList.drop i).take j)
+  (h' : (filterNonterminals u).length = j) :
+    (target.numberNonterminals u i j h h').length = u.length := by
+  induction u using List.reverseRecOn generalizing j with
+  | nil =>
+    simp
+  | append_singleton xs x ih =>
+    simp only [numberNonterminals_append, filterNonterminals_cons, filterNonterminals_nil,
+      List.length_append, ih, List.length_cons, List.length_nil, zero_add, Nat.add_left_cancel_iff]
+    split <;> rfl
+
+@[simp]
+lemma Word.numberNonterminals_single {α V k} (target : Word V k)
+  (s : Symbol α V)
+  (i j : ℕ)
+  (h : filterNonterminals [s] = (target.toList.drop i).take j)
+  (h' : (filterNonterminals [s]).length = j) :
+    target.numberNonterminals [s] i j h h' =
+      match s with
+      | .terminal a => [.terminal a]
+      | .nonterminal n => [.nonterminal ⟨target, ⟨i, by
+        by_contra contra
+        simp only [not_lt] at contra
+        have : target.toList.length ≤ i := by simp [toList, contra]
+        simp [List.drop_of_length_le this] at h ⟩⟩]
+     := by split <;> rfl
+
+@[simp]
+lemma Word.numberNonterminals_filterNonterminals_length {α V k} (target : Word V k)
+  (u : List (Symbol α V))
+  (i j : ℕ)
+  (h : filterNonterminals u = (target.toList.drop i).take j)
+  (h' : (filterNonterminals u).length = j) :
+    (filterNonterminals <| target.numberNonterminals u i j h h').length =
+      (filterNonterminals u).length := by
+  induction u using List.reverseRecOn generalizing j with
+  | nil =>
+    simp
+  | append_singleton xs x ih =>
+    simp only [numberNonterminals_append, filterNonterminals_cons, filterNonterminals_nil,
+      filterNonterminals_append, List.length_append]
+    change
+      let j' := _
+      let h := _
+      let h' := _
+      (filterNonterminals <| target.numberNonterminals _ i j' h h').length + _ = _
+    intro j' h h'
+    --
+    rw [ih j' h h']
+    simp only [Nat.add_left_cancel_iff]
+    split
+    · simp
+    · simp only [List.length_cons, List.length_nil, zero_add]
+      rfl
+
+@[simp]
+lemma filterNonterminals_numberNonterminals_filterNonterminals {α V k} (w : List (Symbol α V))
+  (ww : Word V k) (i j h h') :
+    filterNonterminals
+      (ww.numberNonterminals
+        (List.map (Symbol.nonterminal (T := α)) (filterNonterminals w)) i j h h') =
+    filterNonterminals
+      (ww.numberNonterminals w i j (by simp_all) (by subst h'; simp)) := by
+  induction w using List.reverseRecOn generalizing j with
+  | nil =>
+    rfl
+  | append_singleton xs x ih =>
+    simp only [filterNonterminals_append, filterNonterminals_cons, filterNonterminals_nil,
+      List.map_append, Word.numberNonterminals_append, filterNonterminals_map_nonterminal, ih,
+      Word.numberNonterminals_single, List.append_cancel_left_eq]
+    split <;> rfl
+
+protected def grammar.initial_ {α V T : Type*} (E : EDT0LGrammar α V T) (k : ℕ)
+  (h_index : E.IsIndex k) :
+    Nonterminal V k :=
+  ⟨⟨1, fun _ ↦ E.initial⟩, ⟨0, by
+    have := E.isIndex_k_geq_one h_index
+    cases k <;> simp_all⟩⟩
+
+def grammar {α V T : Type*} (E : EDT0LGrammar α V T) (k : ℕ) (h : E.IsIndex k) :
+    EDT0LGrammar α (Nonterminal V k) T where
+  initial := grammar.initial_ E k h
+  table :=
+    fun t v ↦
+      if can_rewrite : Word.CanRewrite v.word E t then
+        v.rewrite E t can_rewrite
+      else
+        [.nonterminal (grammar.initial_ E k h)]
+
+lemma Word.numberNonterminals_ext {α V k} {ww1 ww2 : Word V k} {i1 i2 j1 j2 : ℕ}
+  {w1 w2 : List (Symbol α V)}
+  {h1 h2 h1' h2'}
+  (hww : ww1 = ww2)
+  (hw : w1 = w2)
+  (hi : i1 = i2) :
+    ww1.numberNonterminals w2 i1 j1 h1 h1' = ww2.numberNonterminals w2 i2 j2 h2 h2' := by
+  subst hww hw hi j1 j2
+  rfl
+
+lemma Word.toNumberedList_length {V k} (w : Word V k) :
+    w.toNumberedList.length = w.toList.length := by simp [toNumberedList, toList]
+
+lemma Word.toNumberedList_eq {α V} {k} (w : Word V k) :
+    w.toNumberedList =
+    filterNonterminals
+      (numberNonterminals (α := α) w (w.toList.map .nonterminal) 0 w.toList.length (by simp)
+        (by simp)) := by
+  let rec go :
+      (i : ℕ) →
+      (hi : i ≤ w.toList.length) →
+      (h : _) → (h' : _) →
+      w.toNumberedList.take i =
+      filterNonterminals
+        (numberNonterminals (α := α) w ((w.toList.take i).map .nonterminal) 0 i h h')
+    | 0, hi, h, h' => by simp
+    | j + 1, hi, h, h' => by
+      have R := go j (Nat.le_of_succ_le hi) (by simp_all)
+        (by
+          simp_all only [List.map_take, filterNonterminals_take_nonterminal, List.drop_zero,
+            List.length_take, inf_of_le_left, inf_eq_left]
+          exact Nat.le_of_succ_le hi )
+      simp only [List.take_add_one, R, List.map_take, List.map_append]
+      simp only [numberNonterminals_append, filterNonterminals_take_nonterminal, List.length_take,
+        min_eq_left (show j ≤ w.toList.length by exact Nat.le_of_succ_le hi), zero_add,
+        filterNonterminals_map_nonterminal, filterNonterminals_append, List.append_cancel_left_eq]
+      unfold toNumberedList
+      simp only [List.getElem?_ofFn]
+      --
+      split
+      · simp only [Option.toList_some]
+        have : j < w.toList.length := Nat.lt_of_lt_of_eq hi rfl
+        simp only [this, getElem?_pos, Option.toList_some, List.map_cons, List.map_nil,
+          List.length_cons, List.length_nil, zero_add]
+        rfl
+      · rename_i h''
+        unfold toList at hi
+        rw [List.length_ofFn] at hi
+        clear * - h'' hi
+        exfalso
+        omega
+  have R := go w.toList.length (Nat.le_refl _) (by simp) (by simp)
+  conv at R => lhs; simp only [← toNumberedList_length, List.take_length]
+  rw [R]
+  simp
+
+lemma grammar_eq_toNumberedList {α V T} (E : EDT0LGrammar α V T) {k} (h : E.IsIndex k)
+  (t : List T) :
+    filterNonterminals ((grammar E k h).rewriteSeq t (grammar E k h).initialWord) =
+    (Word.mk'
+        (w := E.rewriteSeq t E.initialWord)
+        (h _ E.generates_rewriteSeq)).toNumberedList := by
+  induction t using List.reverseRecOn with
+  | nil =>
+    rw [Word.toNumberedList_eq (α := α)]
+    simp only [grammar, rewriteSeq_refl, filterNonterminals_cons, filterNonterminals_nil,
+      Word.mk'_toList, List.map_cons, List.map_nil, List.length_cons, List.length_nil, zero_add,
+      Word.numberNonterminals, List.cons.injEq, and_true]
+    unfold grammar.initial_ Word.mk' initialWord
+    simp only [Fin.coe_ofNat_eq_mod, Nonterminal.mk.injEq, Word.mk.injEq, filterNonterminals_cons,
+      filterNonterminals_nil, List.length_cons, List.length_nil, zero_add]
+    split_ands
+    · exact Fin.one_eq_mk_of_lt _
+    · change let i := _ ; let j := _ ; let f : Fin i → _ := _ ; let g : Fin j → _ := _ ; f ≍ g
+      intro i j f g
+      rw [show g = fun _ ↦ E.initial by unfold g ; ext x ; simp]
+      have : i = j := by
+        subst i j
+        have := E.isIndex_k_geq_one h
+        aesop
+      exact (Fin.heq_fun_iff this).mpr (congrFun rfl)
+    · rw [heq_iff_exists_eq_cast]
+      have := E.isIndex_k_geq_one h
+      use (by
+        simp_all only [ge_iff_le, filterNonterminals_cons, filterNonterminals_nil, List.length_cons,
+          List.length_nil, zero_add]
+        have : 1 % (k + 1) = 1 := by aesop
+        rw [this])
+      refine Fin.ext_iff.mpr ?_
+      rw [Fin.cast_eq_cast']
+      simp
+  | append_singleton xs x ih =>
+    rw [Word.toNumberedList_eq (α := α)]
+    conv => lhs ; simp only [rewriteSeq_seq_append, rewriteSeq_seq_cons, rewriteSeq_refl]
+    rw [filterNonterminals_rewriteWord, ih]
+    simp only [Word.toNumberedList_eq (α := α)]
+    simp only [Word.mk'_toList, rewriteSeq_seq_append, rewriteSeq_seq_cons, rewriteSeq_refl]
+    change
+      let ww := _
+      let ww' := _
+      let w := _
+      let w' := _
+      filterNonterminals (EDT0LGrammar.rewriteWord _ _ (List.map _ (filterNonterminals (
+        Word.numberNonterminals ww (List.map _ w) _ _ _ _)))) =
+      filterNonterminals (Word.numberNonterminals ww' (List.map _ w') _ _ _ _)
+    intro ww ww' w w'
+    --
+    have go (l : ℕ) (hl : l ≤ w.length) (h1 h1' h2 h2') :
+        filterNonterminals (α := α)
+            ((grammar E k h).rewriteWord x
+              (List.map Symbol.nonterminal
+                (filterNonterminals (α := α)
+                  (ww.numberNonterminals (List.map Symbol.nonterminal (w.take l)) 0 l h1 h1')))) =
+          filterNonterminals (α := α)
+            (ww'.numberNonterminals
+              (List.map Symbol.nonterminal
+                (w'.take
+                  (List.length
+                    <| filterNonterminals
+                    <| E.rewriteWord x
+                    <| List.map .nonterminal
+                    <| w.take l)))
+              0
+              (List.length
+                    <| filterNonterminals
+                    <| E.rewriteWord x
+                    <| List.map .nonterminal
+                    <| w.take l)
+              h2 h2') := by
+      clear * - hl
+      induction l with
+      | zero => simp
+      | succ m ih =>
+        if hm : m < w.length then
+          -- have hm' : m + 1 ≤ w.length := by omega
+          have : w[m]?.toList = [w.get ⟨m, hm⟩] := by simp
+          simp only [List.take_add_one, this, List.map_append, Word.numberNonterminals_append,
+            filterNonterminals_append, rewriteWord_append]
+          replace ih := ih (by omega) (by simp [ww, w])
+            (by
+              simp_all only [List.map_take, filterNonterminals_take_nonterminal, List.drop_zero,
+                List.length_take, inf_eq_left, getElem?_pos, Option.toList_some,
+                List.get_eq_getElem]
+              omega)
+            (by simp [w', ww'])
+            (by 
+              simp only [List.map_take, filterNonterminals_take_nonterminal, List.length_take,
+                inf_eq_left, w, w']
+              clear * -
+              conv => rhs ; rw [filterNonterminals_rewriteWord]
+              change
+                let w := _
+                (filterNonterminals (E.rewriteWord _ (List.take _ w))).length ≤
+                  (filterNonterminals (E.rewriteWord _ w)).length
+              intro w
+              conv => rhs; rw [← List.take_append_drop m w]
+              rw [rewriteWord_append]
+              simp)
+          simp only [List.map_take, filterNonterminals_take_nonterminal, List.length_take,
+            min_eq_left (show m ≤ w.length by omega), List.get_eq_getElem, List.map_cons,
+            List.map_nil, filterNonterminals_cons, filterNonterminals_nil, List.length_cons,
+            List.length_nil, zero_add, rewriteWord_cons, rewriteSymbol_nonterminal, rewriteWord_nil,
+            List.append_nil, List.length_append]
+          simp only [List.map_take] at ih
+          rw [ih]
+          simp only [List.take_add, Word.numberNonterminals_append]
+          simp only [filterNonterminals_take_nonterminal, List.length_take, zero_add,
+            filterNonterminals_append]
+          --
+          have :
+            (filterNonterminals (E.rewriteWord x
+              (List.take m (List.map Symbol.nonterminal w)))).length ≤ w'.length := by
+            clear * -
+            subst w'
+            conv => rhs ; rw [filterNonterminals_rewriteWord]
+            change
+              let w := _
+              (filterNonterminals (E.rewriteWord _ (List.take _ w))).length ≤
+                (filterNonterminals (E.rewriteWord _ w)).length
+            intro w
+            conv => rhs; rw [← List.take_append_drop m w]
+            rw [rewriteWord_append]
+            simp
+          simp only [min_eq_left this, List.append_cancel_left_eq]
+          clear * -
+          --
+          simp only [grammar, Nonterminal.rewrite, Word.rewriteNonterminal, Word.numberNonterminals,
+            filterNonterminals_cons, filterNonterminals_nil, List.map_cons, List.map_nil,
+            rewriteWord_cons, rewriteSymbol_nonterminal, Word.canRewrite_rewriteSeq, ↓reduceDIte,
+            rewriteWord_nil, List.append_nil, ww]
+          --
+          have hh1 : w' = filterNonterminals (List.flatMap (E.table x) w) := by
+            simp only [w', w]
+            exact filterNonterminals_rewriteSymbols (E.rewriteSeq xs E.initialWord) E x
+          have hh2 : w = w.take m ++ [w[m]] ++ w.drop (m + 1) := by simp
+          have hh3 :
+            List.take
+              (filterNonterminals (E.table x w[m])).length
+              (List.drop
+                (filterNonterminals
+                  (E.rewriteWord x
+                    (List.take m (List.map Symbol.nonterminal w)))).length
+                  (List.map (Symbol.nonterminal (T := α)) w')) =
+              List.map .nonterminal (filterNonterminals (E.table x w[m])) := by
+            rw [hh1]
+            conv => lhs; arg 2; arg 2; rw [hh2]
+            simp only [List.flatMap_append]
+            simp only [List.flatMap_cons, List.flatMap_nil, List.append_nil, List.append_assoc,
+              filterNonterminals_append, List.map_append]
+            change
+              let a := _
+              let b := _
+              let ii := _
+              let jj := _
+              (List.take ii <| List.drop jj <| a ++ (b ++ _)) = _
+            intro a b ii jj
+            --
+            have : jj = a.length := by
+              subst a jj
+              simp only [List.length_map]
+              apply congrArg List.length
+              rw [← List.map_take, rewriteWord, List.flatMap_map]
+              simp
+            rw [this]
+            simp only [List.drop_left']
+            clear this
+            --
+            have : ii = b.length := by
+              subst ii b
+              simp
+            rw [this]
+            simp only [List.take_left']
+            clear this
+            --
+            subst b
+            rfl
+          --
+          simp only [hh3]
+          simp only [filterNonterminals_map_nonterminal]
+          --
+          conv => lhs; arg 1; arg 2; arg 3; change w[m]
+          simp only [filterNonterminals_numberNonterminals_filterNonterminals]
+          --
+          refine congrArg filterNonterminals ?_
+          --
+          change 
+            let ww'2 := _
+            Word.numberNonterminals ww'2 _ _ _ _ _ = _
+          intro ww'2
+          have : ww' = ww'2 := by
+            subst ww' ww'2
+            unfold Word.rewrite Word.mk'
+            simp only [Word.mk.injEq, Fin.mk.injEq]
+            split_ands
+            · simp only [Word.rewriteLength, Word.rewriteFilterNonterminals, Word.toList,
+                List.ofFn_get]
+              exact Nat.succ_inj.mp (congrArg Nat.succ (congrArg List.length hh1))
+            · simp only [Word.rewriteLength, Word.rewriteFilterNonterminals, Word.toList]
+              rw [List.ofFn_get, filterNonterminals_rewriteSymbols]
+          simp only [this]
+          refine Word.numberNonterminals_ext rfl rfl ?_
+          simp only [Word.rewriteFilterNonterminalsTake, Word.toList, Word.mk', List.ofFn_get]
+          refine congrArg List.length ?_
+          subst w
+          clear * -
+          rw [filterNonterminals_rewriteWord]
+          induction E.rewriteSeq xs E.initialWord generalizing m with
+          | nil =>
+            simp
+          | cons y ys ih =>
+            simp only [filterNonterminals_cons, filterNonterminals_take_nonterminal, List.map_take]
+            split
+            · simp [ih]
+            · if hm : m > 0 then
+                rw [List.map_cons]
+                repeat rw [List.take_cons (i := m) (h := hm)]
+                simp [ih]
+              else
+                simp_all
+        else
+          exfalso
+          omega
+    replace go := go w.length
+      (by simp)
+      (by simp [w, ww])
+      (by simp [w])
+      (by simp [w, w', ww'])
+      (by
+        simp only [List.take_length, List.map_take, filterNonterminals_take_nonterminal,
+          List.length_take, inf_eq_left, w, w']
+        rw [@Nat.le_iff_lt_or_eq]
+        right
+        apply congrArg List.length
+        exact Eq.symm (filterNonterminals_rewriteWord (E.rewriteSeq xs E.initialWord) E x) )
+    simp only [List.take_length] at go
+    rw [go]
+    have :
+      (filterNonterminals (E.rewriteWord x (List.map Symbol.nonterminal w))).length =
+        w'.length := by
+      unfold w w'
+      rw [filterNonterminals_rewriteWord]
+      simp only [filterNonterminals_map_nonterminal]
+      apply congrArg List.length
+      exact Eq.symm (filterNonterminals_rewriteWord (E.rewriteSeq xs E.initialWord) E x)
+    simp [this]
+    rfl
+  -- induction t using List.reverseRecOn with
+  -- | nil =>
+  --   simp only [rewriteSeq_refl, filterNonterminals_cons, filterNonterminals_nil,
+  --     Word.toNumberedList]
+  --   -- split_ands
+  --   -- · aesop
+  --   -- · have : 1 % (k + 1) = 1 := by aesop
+  --   --   have : Fin (1 % (k+1)) =
+  --   --       Fin (filterNonterminals (α := α) [.nonterminal E.initial]).length := by tauto
+  --   --   rw [this]
+  --   --   simp only [heq_eq_eq]
+  --   --   change _ = [E.initial].get
+  --   --   ext1 x
+  --   --   simp
+  --   -- · have : 1 % (k + 1) = 1 := by aesop
+  --   --   have h : Fin (1 % (k + 1)) =
+  --   --       Fin (filterNonterminals (α := α) [.nonterminal E.initial]).length := by tauto
+  --   --   exact (Fin.heq_ext_iff this).mpr rfl
+  --   
+  --   sorry
+  -- | append_singleton ts t ih =>
+  --   simp only [rewriteSeq_seq_append, rewriteSeq_seq_cons, rewriteSeq_refl]
+  --   rw [filterNonterminals_rewriteSymbols, ih]
+  --   unfold Word.toNumberedList grammar
+  --   change
+  --     let x := _
+  --     let y := _
+  --     let f : _ → _ := _
+  --     filterNonterminals (List.flatMap f x) = y
+  --   intro x y f
+  --   --
+  --   have go (i : ℕ) :
+  --       filterNonterminals (List.flatMap f (x.take i)) =
+  --       y.take (List.length <| filterNonterminals (List.flatMap f (x.take i))) := by
+  --     induction i with
+  --     | zero =>
+  --       rfl
+  --     | succ j ih =>
+  --       rw [List.take_add]
+  --       simp only [List.flatMap_append, filterNonterminals_append, List.length_append]
+  --       rw [ih]
+  --       conv => rhs; rw [List.take_add]
+  --       change let a := _ ; let b := _ ; a ++ _ = b ++ _
+  --       intro a b
+  --       have : a = b := by subst a b; simp
+  --       rw [this, List.append_cancel_left_eq]
+  --       clear this a b
+  --       if hj : j < x.length then
+  --         have : List.take 1 (List.drop j x) = [x.get ⟨j, hj⟩] :=
+  --           List.take_one_drop_eq_of_lt_length hj
+  --         simp only [this]
+  --         simp only [List.get_eq_getElem, List.flatMap_cons, List.flatMap_nil, List.append_nil,
+  --           List.length_take]
+  --         subst x y f
+  --         simp only [List.getElem_ofFn, List.length_ofFn]
+  --         simp only [Word.canRewrite_rewriteSeq, ↓reduceDIte]
+  --         clear * - h
+  --
+  --         sorry
+  --       else
+
+-- lemma p2_imp_canRewrite {α V T k} (ts : List T) (t : T)
+--   (E : EDT0LGrammar α V T)
+--   (h : E.IsIndex k)
+--   (hu : List.length (filterNonterminals (E.rewriteSeq ts E.initialWord)) ≤ k)
+--   (p2 : filterNonterminals ((grammar E k h).rewriteSeq ts (grammar E k h).initialWord) =
+--           (Word.mk' hu).toNumberedList) :
+--     (Word.mk' hu).CanRewrite E t := by
+--   unfold Word.CanRewrite Word.rewriteLength Word.rewriteFilterNonterminals
+--   have p2' := congrArg (List.map fun x ↦ x.unlabel) p2
+--   unfold Word.toNumberedList at p2'
+--   simp only [List.map_ofFn] at p2'
+--   change let f : _ → _ := _ ; _ = List.ofFn f at p2'
+--   extract_lets f at p2'
+--   have : f = (Word.mk' hu).get := rfl
+--   rw [this] at p2'
+--   change _ = (Word.mk' hu).toList at p2'
+--   -- rw [← p2']
+--   -- simp only [gt_iff_lt]
+--   --
+--   have go (x : List (Symbol α (Nonterminal V k))) :
+--       filterNonterminals
+--         (List.flatMap (E.table t) (List.map (fun x ↦ x.unlabel) (filterNonterminals x))) =
+--       (List.map (fun x ↦ x.unlabel)
+--         (filterNonterminals ((grammar E k h).rewriteWord t x))) := by
+--     clear * -
+--     induction x with
+--     | nil =>
+--       rfl
+--     | cons x xs ih =>
+--       simp only [filterNonterminals_cons, rewriteWord_cons, filterNonterminals_append,
+--         List.map_append]
+--       split
+--       · simp [ih]
+--       · simp only [List.map_cons, List.flatMap_cons, filterNonterminals_append, ih,
+--           rewriteSymbol_nonterminal, List.append_cancel_right_eq]
+--         rename_i v
+--         sorry
+  --
+  --
+  -- unfold filterNonterminals
+  -- simp [List.map_filterMap]
+  --
+  -- sorry
+
+lemma grammar_normalForm {α V T : Type*} (E : EDT0LGrammar α V T) (k : ℕ)
+  (h : E.IsIndex k) (s : List T) :
+    UnlabelWord ((grammar E k h).rewriteSeq s (grammar E k h).initialWord) =
+    (E.rewriteSeq s E.initialWord) := by
+  induction s using List.reverseRecOn with
+  | nil =>
+    rfl
+  | append_singleton xs x ih =>
+      simp only [rewriteSeq_seq_append, rewriteSeq_seq_cons, rewriteSeq_refl]
+      have go (i : ℕ) :
+          UnlabelWord
+              ((grammar E k h).rewriteWord x
+                (((grammar E k h).rewriteSeq xs (grammar E k h).initialWord).take i)) =
+          E.rewriteWord x
+              (UnlabelWord
+                (((grammar E k h).rewriteSeq xs (grammar E k h).initialWord).take i)) := by
+        induction i with
+        | zero =>
+          rfl
+        | succ i ih =>
+          rw [List.take_add_one]
+          if hi : i < ((grammar E k h).rewriteSeq xs (grammar E k h).initialWord).length then
+            simp only [getElem?_pos, Option.toList_some, rewriteWord_append, rewriteWord_cons,
+              rewriteWord_nil, List.append_nil, unlabelWord_append, unlabelWord_cons,
+              List.append_cancel_left_eq, ih, hi, unlabelWord_nil, rewriteWord_nil,
+              List.append_nil]
+            split <;> rename_i heq <;> rw [heq]
+            · simp
+            · rename_i v
+              have hh : .nonterminal v ∈ (grammar E k h).rewriteSeq
+                  xs (grammar E k h).initialWord := List.mem_of_getElem heq
+              rw [← filterNonterminals_mem_iff, grammar_eq_toNumberedList, Word.toNumberedList]
+                at hh
+              simp only [List.mem_ofFn] at hh
+              --
+              have : v.word.CanRewrite E x := by
+                obtain ⟨ii, rfl⟩ := hh
+                unfold Word.CanRewrite Word.rewriteLength Word.rewriteFilterNonterminals
+                simp only [Word.mk'_toList]
+                --
+                have (w : List V) :
+                    List.flatMap (E.table x) w = E.rewriteWord x (w.map .nonterminal) := by
+                  simp [rewriteWord, List.flatMap_map]
+                simp only [this, gt_iff_lt]
+                clear this
+                --
+                rw [← filterNonterminals_rewriteWord,
+                  ← rewriteSeq_seq_single,
+                  ← rewriteSeq_seq_append]
+                --
+                have := h (E.rewriteSeq (xs ++ [x]) E.initialWord) E.generates_rewriteSeq
+                exact Nat.lt_succ_of_le this
+              simp only [grammar, Nonterminal.rewrite, Word.rewriteNonterminal,
+                rewriteSymbol_nonterminal, this, ↓reduceDIte, unlabelWord_numberNonterminals]
+              rfl
+          else
+            simp_all
+      have := go ((grammar E k h).rewriteSeq xs (grammar E k h).initialWord).length
+      simp only [List.take_length] at this
+      rw [this]
+      refine congrArg (E.rewriteWord x) ?_
+      exact ih
+
+lemma grammar_language_eq {α V T} (E : EDT0LGrammar α V T) (k : ℕ) (h : E.IsIndex k) :
+    E.language = (grammar E k h).language := by
+  ext1 w
+  simp only [language_mem_iff, generates_iff_rewriteSeq]
+  --
+  let rec go : (w' : List (Symbol α (Nonterminal V k))) → (w : List α) →
+      UnlabelWord w' = List.map Symbol.terminal w →
+      w' = List.map Symbol.terminal w
+    | [],[], h => rfl
+    | a::as, b::bs, h => by
+      simp_all only [unlabelWord_cons, List.map_cons, List.cons.injEq]
+      obtain ⟨h1,h2⟩ := h
+      split at h1
+      · simp_all only [Symbol.terminal.injEq, true_and]
+        exact go as bs h2
+      · simp_all 
+    | _::_,[],h => by
+      simp at h
+    | [],_::_,h => by
+      change [] = _ at h
+      simp at h
+  --
+  constructor
+  · intro h'
+    obtain ⟨s, h'⟩ := h'
+    use s
+    have p1 := grammar_normalForm E k h s
+    rw [h'] at p1
+    clear * - p1
+    change let w' := _ ; w' = _
+    intro w'
+    change UnlabelWord w' = _ at p1
+    exact go w' w p1
+  · intro h'
+    obtain ⟨s, h'⟩ := h'
+    use s
+    have p1 := grammar_normalForm E k h s
+    rw [h'] at p1
+    rw [← p1]
+    clear * -
+    induction w with
+    | nil => rfl
+    | cons x xs ih => simp_all
+
+lemma grammar_isLULT {α V T} [DecidableEq V] (E : EDT0LGrammar α V T) (k : ℕ) (h : E.IsIndex k) :
+    (grammar E k h).IsLULT := by
+  intro w hw
+  simp only [language_mem_iff, generates_iff_rewriteSeq] at hw
+  obtain ⟨s, hw⟩ := hw
+  use s
+  constructor
+  · exact hw
+  --
+  intro v i hi
+  left
+  rw [grammar_eq_toNumberedList]
+  --
+  change let ww := _ ; List.count v (Word.toNumberedList ww) ≤ 1
+  intro ww
+  have := Word.toNumberedList_nodup ww
+  rw [List.nodup_iff_count] at this
+  exact this _
+
+end FiEDT0L2LULT
+end EDT0LGrammar
+
+theorem Language.isFiniteIndexEDT0L_imp_isLULT {α} (L : Language α) (h : L.IsFiniteIndexEDT0L) :
+    L.IsLULT := by
+  classical
+  obtain ⟨k, ⟨n, m, E, h, rfl⟩⟩ := h
+  rw [EDT0LGrammar.FiEDT0L2LULT.grammar_language_eq E k h]
+  refine EDT0LGrammar.lult_language_isLULT (EDT0LGrammar.FiEDT0L2LULT.grammar E k h) ?_
+  exact EDT0LGrammar.FiEDT0L2LULT.grammar_isLULT E k h
