LSystems/FiniteIndexEDT0L/Mapped.lean
@@ -1,0 +1,46 @@
+/-
+Copyright (c) 2026 Alex Bishop. All rights reserved.
+Released under Apache 2.0 license as described in the file LICENSE.
+Author: Alex Bishop
+-/
+module
+
+public import LSystems.EDT0L.Mapped
+public import LSystems.FiniteIndexEDT0L.Defs
+
+@[expose] public section
+
+namespace EDT0LGrammar
+
+lemma map_isIndex {α V T α'} (f : α → α') (E : EDT0LGrammar α V T) {k} (h : E.IsIndex k) :
+    (E.Mapped f).IsIndex k := by
+  intro w hw
+  rw [generates_iff_rewriteSeq] at hw
+  obtain ⟨s, rfl⟩ := hw
+  replace h := h (E.rewriteSeq s E.initialWord) E.generates_rewriteSeq
+  simp only [mapped_initialWord, mapWord_cons, mapWord_nil, ge_iff_le]
+  have h' := mapped_rewriteSeq f E s [.nonterminal E.initial]
+  conv at h' =>
+    lhs
+    unfold mapWord
+    rw [List.map_singleton]
+    simp only
+  rw [h']
+  simpa using h
+
+end EDT0LGrammar
+
+lemma Language.map_isEDT0LOfIndex {α α'} (f : α → α') (L : Language α)
+  {k} (h : L.IsEDT0LOfIndex k) :
+    (L.map f).IsEDT0LOfIndex k := by
+  obtain ⟨n,m,E,h,rfl⟩ := h
+  use n,m,E.Mapped f, EDT0LGrammar.map_isIndex f E h
+  exact EDT0LGrammar.mapped_language f E
+
+lemma Language.map_isFiniteIndexEDT0L {α α'} (f : α → α') (L : Language α)
+  (h : L.IsFiniteIndexEDT0L) :
+    (L.map f).IsFiniteIndexEDT0L := by
+  obtain ⟨k,h⟩ := h
+  use k
+  exact map_isEDT0LOfIndex f L h
+
