LSystems/FiniteIndexEDT0L/RegularLanguage.lean
@@ -3,64 +3,38 @@ Copyright (c) 2025 Alex Bishop. All rights reserved.
 Released under Apache 2.0 license as described in the file LICENSE.
 Author: Alex Bishop
 -/
-import LSystems.EDT0L.Defs
-import LSystems.EDT0L.RegularLanguage
-import LSystems.FiniteIndexEDT0L.Defs
+module
+
+public import LSystems.EDT0L.Defs
+public import LSystems.EDT0L.RegularLanguage
+public import LSystems.FiniteIndexEDT0L.Defs
+
+import LSystems.EDT0L.RewriteSequence
+
+@[expose] public section
 
 namespace EDT0LGrammar
 
-lemma terminal_word_count {α V : Type*} (w : List α) :
-    List.countP (@SymbolIsNonterminal α V) (List.map .terminal w) = 0 := by
-  induction w with
-  | nil =>
-    simp only [List.map_nil, List.countP_nil]
-  | cons a as ih =>
-    simp only [List.map_cons, List.countP_cons]
-    conv =>
-      lhs ; rhs
-      unfold SymbolIsNonterminal
-      change 0
-    simp only [add_zero]
-    exact ih
-
-theorem regular_languages_are_fi_edt0l {α : Type*} [Fintype α] (L : Language α) :
-    L.IsRegular → L.IsEDT0LOfIndex 1 := by
-  unfold Language.IsRegular
-  intro h
-  have ⟨ _, _, M, h₁ ⟩ := h
-  --
-  let data := DFAData.mk M
-  have h₂ := data.languages_are_identical
-
-  let E := data.grammar
-
-  have h₃ : E.language = M.accepts := by
-    unfold EDT0LGrammar.language
-    unfold DFA.accepts
-    unfold DFA.acceptsFrom
-    subst h₁
-    simp_all only [exists_const_iff, data, E]
-
-  rw [h₁] at h₃
-  rw [← h₃]
-  apply E.fi_edt0l_grammars_generate_fi_edt0l_languages'
-  
-  intro w h
-  replace ⟨u, h⟩ := data.generated_words w h
-  cases h with
-  | inl h =>
-    replace h := h.left
+lemma regular_isEDT0LOfIndex_one {α σ} [DecidableEq σ] (dfa : DFA α σ) :
+    (Regular dfa).IsIndex 1 := by
+  intro w hw
+  rw [regular_generates_iff] at hw
+  cases hw with
+  | processing u h | done u h h_accept =>
     subst h
-    rw [terminal_word_count]
-    simp only [zero_le]
-  | inr h =>
-    subst h
-    simp only [List.countP_append, terminal_word_count, zero_add]
-    unfold SymbolIsNonterminal
-    simp only [List.countP_singleton]
-    split 
-    · rfl
-    · simp only [zero_le]
+    simp
 
 end EDT0LGrammar
+
+theorem Language.isReguar_imp_isEDT0LOfIndex_one {α : Type*} [Finite α] (L : Language α) :
+    L.IsRegular → L.IsEDT0LOfIndex 1 := by
+  classical
+  have : Fintype α := Fintype.ofFinite α
+  intro h
+  replace ⟨σ, finσ, dfa, h⟩ := h
+  rw [← EDT0LGrammar.regular_eq_dfa dfa] at h
+  rw [← h]
+  unfold Language.IsEDT0LOfIndex
+  apply EDT0LGrammar.isIndex_imp_language_isEDT0LOfIndex
+  exact EDT0LGrammar.regular_isEDT0LOfIndex_one dfa
 
