LSystems/FiniteIndexEDT0L/Union.lean
@@ -3,85 +3,74 @@ Copyright (c) 2025 Alex Bishop. All rights reserved.
 Released under Apache 2.0 license as described in the file LICENSE.
 Author: Alex Bishop
 -/
-import LSystems.EDT0L.Defs
-import LSystems.EDT0L.Union
-import LSystems.FiniteIndexEDT0L.Defs
+module
+
+public import LSystems.EDT0L.Defs
+public import LSystems.EDT0L.Union
+public import LSystems.FiniteIndexEDT0L.Defs
+
+@[expose] public section
 
 namespace EDT0LGrammar
 
-namespace UnionData
+@[simp]
+lemma filterNonterminals_map_symbol_lhs_length {α V₀ V₁} (s : List (Symbol α V₀)) :
+    (filterNonterminals (List.map (Union.map_symbol_lhs (V₁ := V₁)) s)).length =
+      (filterNonterminals s).length := by
+  induction s with
+  | nil =>
+    rfl
+  | cons x xs ih =>
+    simp only [List.map_cons, filterNonterminals_cons]
+    split <;> rename_i heq <;> split <;> simp [ih, Union.map_symbol_lhs] at ⊢ heq
 
-section helpers
-variable {α V₀ V₁ : Type*}
+@[simp]
+lemma filterNonterminals_map_symbol_rhs_length {α V₀ V₁} (s : List (Symbol α V₁)) :
+    (filterNonterminals (List.map (Union.map_symbol_rhs (V₀ := V₀)) s)).length =
+      (filterNonterminals s).length := by
+  induction s with
+  | nil =>
+    rfl
+  | cons x xs ih =>
+    simp only [List.map_cons, filterNonterminals_cons]
+    split <;> rename_i heq <;> split <;> simp [ih, Union.map_symbol_rhs] at ⊢ heq
 
-lemma extend_alphabet₀_is_nonterminal (s : Symbol α V₀) :
-    SymbolIsNonterminal s = (SymbolIsNonterminal <| @extend_alphabet₀ α V₀ V₁ <| s) := by
-  unfold extend_alphabet₀
-  split <;> rfl
-
-lemma extend_alphabet₁_is_nonterminal (s : Symbol α V₁) :
-    SymbolIsNonterminal s = (SymbolIsNonterminal <| @extend_alphabet₁ α V₀ V₁ <| s) := by
-  unfold extend_alphabet₁
-  split <;> rfl
-
-lemma extend_alphabet₀_map_count (w : List (Symbol α V₀)) :
-    w.countP SymbolIsNonterminal
-    = (w.map (@extend_alphabet₀ α V₀ V₁)).countP SymbolIsNonterminal := by
-  induction w with
-  | nil => simp only [List.countP_nil, List.map_nil]
-  | cons α as ih =>
-    simp only [List.map_cons, List.countP_cons]
-    rw [ih]
-    rw [extend_alphabet₀_is_nonterminal]
-
-lemma extend_alphabet₁_map_count (w : List (Symbol α V₁)) :
-    w.countP SymbolIsNonterminal
-    = (w.map (@extend_alphabet₁ α V₀ V₁)).countP SymbolIsNonterminal := by
-  induction w with
-  | nil => simp only [List.countP_nil, List.map_nil]
-  | cons a as ih =>
-    simp only [List.map_cons, List.countP_cons]
-    rw [ih]
-    rw [extend_alphabet₁_is_nonterminal]
-
-end helpers
-
-variable {α V₀ T₀ V₁ T₁ : Type*} [Fintype V₀] [Fintype T₀] [Fintype V₁] [Fintype T₁]
-variable (data : @UnionData α V₀ T₀ V₁ T₁ _ _ _ _)
-
-theorem closed_under_union' {k₁ k₂ : ℕ}
-  (h₀ : data.E₀.IsIndex k₁)
-  (h₁ : data.E₁.IsIndex k₂) :
-    data.grammar.IsIndex (Nat.max k₁ k₂) := by
-  --
-  unfold IsIndex
-  intro w h
-  replace h := data.basic_property w h
-  obtain rfl | ⟨u, ⟨rfl, h⟩⟩ | ⟨u, ⟨rfl, h⟩⟩ := h
-  · calc List.countP SymbolIsNonterminal [Symbol.nonterminal data.grammar.initial]
-      _ = 1 := SymbolIsNonterminal_single_nonterminal _
-      _ ≤ k₁ := index_at_least_one _ h₀
-      _ ≤ Nat.max k₁ k₂ := le_sup_left
-  · rw [← extend_alphabet₀_map_count]
-    replace h := generates_implies_le_index data.E₀ u h₀ h
-    simp only [le_sup_iff, h, true_or]
-  · rw [← extend_alphabet₁_map_count]
-    replace h := generates_implies_le_index data.E₁ u h₁ h
-    simp only [le_sup_iff, h, or_true]
-
-end UnionData
-
-theorem finite_index_closed_under_union {α : Type*} {k₁ k₂ : ℕ} (L₁ L₂ : Language α)
-  (h₁ : L₁.IsEDT0LOfIndex k₁)
-  (h₂ : L₂.IsEDT0LOfIndex k₂) :
-    (L₁ + L₂).IsEDT0LOfIndex (Nat.max k₁ k₂) := by
-  have ⟨_, _ , E₁, f₁, P₁⟩ := h₁
-  have ⟨_, _ , E₂, f₂, P₂⟩ := h₂
-  let union_data := UnionData.mk E₁ E₂
-  have h₃ := union_data.defines_union
-  have h₄ := union_data.closed_under_union' f₁ f₂
-  have ⟨n,m,E',h',P'⟩ := union_data.grammar.fi_edt0l_grammars_generate_fi_edt0l_languages' h₄
-  use n, m, E', h'
-  rw [P', h₃, P₁, P₂]
+theorem Union.isIndex {α V₀ T₀ V₁ T₁ : Type*}
+  (E₀ : EDT0LGrammar α V₀ T₀)
+  {k₀} (h₀ : E₀.IsIndex k₀)
+  (E₁ : EDT0LGrammar α V₁ T₁)
+  {k₁} (h₁ : E₁.IsIndex k₁) :
+    (Union E₀ E₁).IsIndex (Nat.max k₀ k₁) := by
+  intro w hw
+  rw [Union.generates_iff] at hw
+  cases hw with
+  | init h =>
+    subst h
+    simp [isIndex_k_geq_one E₀ h₀, isIndex_k_geq_one E₁ h₁]
+  | lhs s h1 h2 =>
+    subst h1
+    simp only [le_sup_iff]
+    left
+    have h₀ := h₀ _ h2
+    simp [h₀]
+  | rhs s h1 h2 =>
+    subst h1
+    simp only [le_sup_iff]
+    right
+    have h₁ := h₁ _ h2
+    simp [h₁]
 
 end EDT0LGrammar
+
+theorem Language.isEDT0LOfIndex_union {α} (L₁ L₂ : Language α) {k₁ k₂}
+  (h₁ : L₁.IsEDT0LOfIndex k₁)
+  (h₂ : L₂.IsEDT0LOfIndex k₂) :
+    (L₁ + L₂).IsEDT0LOfIndex (max k₁ k₂):= by
+  have ⟨_, _ , E₁, PP1, P₁⟩ := h₁
+  have ⟨_, _ , E₂, PP2, P₂⟩ := h₂
+  have h := EDT0LGrammar.Union.defines_union E₁ E₂
+  rw [P₁, P₂] at h
+  rw [← h]
+  refine EDT0LGrammar.isIndex_imp_language_isEDT0LOfIndex (E₁.Union E₂) (max k₁ k₂) ?_
+  exact EDT0LGrammar.Union.isIndex E₁ PP1 E₂ PP2
+
