LSystems/StringTransducer.lean
@@ -1,6 +1,0 @@
-/-
-Copyright (c) 2025 Alex Bishop. All rights reserved.
-Released under Apache 2.0 license as described in the file LICENSE.
-Author: Alex Bishop
--/
-import LSystems.StringTransducer.Defs
